I have created a new directory
   certicoq/Randy_8.5beta2/RandyWorking

containing my 4 previous directories (Common bits, L1, L2 and L3).

This new directory is for coq 8.5beta2 as opam-ized by Matthieu.
Everything from before works except one lemma in each of L1, L2 and
l3.  (The same lemma for each language respectively).  This is because
a call to [Functional Scheme] that used to work in 8.4 no longer does.
I'm working on an alternative proof of this lemma, or maybe someone
will fix the [Functional Scheme] command.

L3 has unary applications and eta-expanded constructors.  L3 is not
yet proven correct w.r.t. L2, but all tests work.

reify/template-coq-univ-is-type/theories/Ast.v
@@ -1,8 +1,12 @@
 Require Import Coq.Strings.String.
 Require Import Coq.PArith.BinPos.
 
-Definition universe := positive.
+Definition universe := Type (* positive *).
 Definition ident := string.
+Record const := mk_const
+{ constPath : list ident
+; constName : ident
+}.
 
 Inductive sort : Type :=
 | sProp
@@ -22,7 +26,7 @@ Inductive cast_kind : Type :=
 | RevertCast.
 
 Inductive inductive : Type :=
-| mkInd : string -> nat -> inductive.
+| mkInd : const -> nat -> inductive.
 
 Record def (term : Type) : Type := mkdef
 { dname : name (** the name (note, this may mention other definitions **)
@@ -45,7 +49,7 @@ Inductive term : Type :=
 | tLambda    : name -> term (** the type **) -> term -> term
 | tLetIn     : name -> term (** the type **) -> term -> term -> term
 | tApp       : term -> list term -> term
-| tConst     : string -> term
+| tConst     : const -> term
 | tInd       : inductive -> term
 | tConstruct : inductive -> nat -> term
 | tCase      : nat (* # of parameters *) -> term (** type info **) -> term -> list term -> term
