Randy_8.5beta2/RandyWorking/L1_MalechaQuoted/awndEval.v
@@ -1,0 +1,1227 @@
+(** An alternative definition of wndEval that is extensionally
+*** equivalent for well-formed programs
+**)
+
+Add LoadPath "../common" as Common.
+Add LoadPath "." as L1.
+Require Import Lists.List.
+Require Import Strings.String.
+Require Import Strings.Ascii.
+Require Import Arith.Compare_dec.
+Require Import Relations.Relation_Operators.
+Require Import Relations.Operators_Properties.
+Require Import Setoid.
+Require Import L1.term.
+Require Import L1.program.
+Require Import L1.wndEval.
+
+Local Open Scope string_scope.
+Local Open Scope bool.
+Local Open Scope list.
+Set Implicit Arguments.
+
+(*** alrernative non-deterministic small step evaluation relation ***)
+Inductive awndEval (p:environ) : Term -> Term -> Prop :=
+(** contraction steps **)
+| aConst: forall (s:string) (t:Term),
+            LookupDfn s p t -> awndEval p (TConst s) t
+| aBeta: forall (nm:name) (ty bod arg:Term) (args:Terms),
+           awndEval p (TApp (TLambda nm ty bod) arg args)
+                   (whBetaStep bod arg args)
+     (* note: [instantiate] is total *)
+| aLetIn: forall (nm:name) (dfn ty bod:Term),
+            awndEval p (TLetIn nm dfn ty bod) (instantiate dfn 0 bod)
+     (* Case argument must be in Canonical form *)
+     (* np is the number of parameters of the datatype *)
+| aCase0: forall (n:nat) (ty s:Term) (i:inductive) (brs:Terms),
+            whCaseStep n tnil brs = Some s ->
+            awndEval p (TCase 0 ty (TConstruct i n) brs) s
+| aCasen: forall (np:nat) (ty s arg:Term) (i:inductive)
+                 (args brs ts:Terms) (n:nat),
+            tskipn np (tcons arg args) = Some ts ->
+            whCaseStep n ts brs = Some s ->
+            awndEval p (TCase np ty (TApp (TConstruct i n) arg args) brs) s
+| aFix: forall (dts:Defs) (m:nat) (arg s:Term) (args:Terms),
+          whFixStep dts m (tcons arg args) = Some s ->
+          awndEval p (TApp (TFix dts m) arg args) s
+| aCast: forall t ck ty, awndEval p (TCast t ck ty) t
+(** congruence steps **)
+(** no xi rules: sLambdaR, sProdR, sLetInR,
+*** no congruence on Case branches or Fix ***)
+| aAppFn:  forall (t r arg:Term) (args:Terms),
+              awndEval p t r ->
+              awndEval p (TApp t arg args) (mkApp r (tcons arg args))
+| aAppArg: forall (t arg brg:Term) (args:Terms),
+              awndEval p arg brg ->
+              awndEval p (TApp t arg args) (TApp t brg args)
+| aAppArgs: forall (t arg:Term) (args brgs:Terms),
+              awndEvals p args brgs ->
+              awndEval p (TApp t arg args) (TApp t arg brgs)
+| aProdTy:  forall (nm:name) (t1 t2 bod:Term),
+              awndEval p t1 t2 ->
+              awndEval p (TProd nm t1 bod) (TProd nm t2 bod)
+| aLamTy:   forall (nm:name) (t1 t2 bod:Term),
+              awndEval p t1 t2 ->
+              awndEval p (TLambda nm t1 bod) (TLambda nm t2 bod)
+| aLetInTy: forall (nm:name) (t1 t2 d bod:Term),
+              awndEval p t1 t2 ->
+              awndEval p (TLetIn nm d t1 bod) (TLetIn nm d t2 bod)
+| aLetInDef:forall (nm:name) (t d1 d2 bod:Term),
+              awndEval p d1 d2 ->
+              awndEval p (TLetIn nm d1 t bod) (TLetIn nm d2 t bod)
+| aCaseTy:  forall (np:nat) (ty uy mch:Term) (brs:Terms),
+              awndEval p ty uy ->
+              awndEval p (TCase np ty mch brs) (TCase np uy mch brs)
+| aCaseArg: forall (np:nat) (ty mch can:Term) (brs:Terms),
+              awndEval p mch can ->
+              awndEval p (TCase np ty mch brs) (TCase np ty can brs)
+| aCaseBrs: forall (np:nat) (ty mch:Term) (brs brs':Terms),
+              awndEvals p brs brs' ->
+              awndEval p (TCase np ty mch brs) (TCase np ty mch brs')
+with awndEvals (p:environ) : Terms -> Terms -> Prop :=
+     | aaHd: forall (t r:Term) (ts:Terms), 
+               awndEval p t r ->
+               awndEvals p (tcons t ts) (tcons r ts)
+     | aaTl: forall (t:Term) (ts ss:Terms),
+               awndEvals p ts ss ->
+               awndEvals p (tcons t ts) (tcons t ss).
+Hint Constructors awndEval awndEvals.
+Scheme awndEval1_ind := Induction for awndEval Sort Prop
+  with awndEvals1_ind := Induction for awndEvals Sort Prop.
+Combined Scheme awndEvalEvals_ind from awndEval1_ind, awndEvals1_ind.
+
+Definition no_awnd_step (p:environ) (t:Term) : Prop :=
+  no_step (awndEval p) t.
+Definition no_awnds_step (p:environ) (ts:Terms) : Prop :=
+  no_step (awndEvals p) ts.
+
+Lemma awndEval_tappendl:
+  forall p bs cs, awndEvals p bs cs ->
+  forall ds, awndEvals p (tappend bs ds) (tappend cs ds).
+Proof.
+  induction 1; intros.
+  - constructor. assumption.
+  - simpl. apply aaTl. apply IHawndEvals.
+Qed.
+
+Lemma wndEval_tappendr:
+  forall p bs cs, awndEvals p bs cs ->
+  forall ds, awndEvals p (tappend ds bs) (tappend ds cs).
+Proof.
+  intros p bs cs h ds. induction ds; simpl.
+  - assumption.
+  - apply aaTl. apply IHds.
+Qed.
+
+Lemma awndEval_Lam_inv:
+  forall p nm tp bod s,
+    awndEval p (TLambda nm tp bod) s ->
+    exists tp', awndEval p tp tp' /\ s = (TLambda nm tp' bod).
+intros p nm tp bod s h. inversion_Clear h.
+- exists t2. split; [assumption | reflexivity].
+Qed.
+
+Lemma awndEval_Prod_inv:
+  forall p nm tp bod s,
+    awndEval p (TProd nm tp bod) s ->
+    exists tp', awndEval p tp tp' /\ s = (TProd nm tp' bod).
+intros p nm tp bod s h. inversion_Clear h.
+- exists t2. split; [assumption | reflexivity].
+Qed.
+
+Lemma awndEval_Cast_inv:
+  forall p tm ck ty s,
+    awndEval p (TCast tm ck ty) s -> tm = s.
+inversion 1. reflexivity.
+Qed.
+
+Lemma awndEval_mkApp_mkApp:
+  forall p s u, awndEval p s u -> WFaEnv p -> WFapp s ->
+  forall a1 args,
+     awndEval p (mkApp s (tcons a1 args)) (mkApp u (tcons a1 args)).
+Proof.
+  induction 1; simpl; intros hp; intros hs; intros;
+  inversion hs; subst; auto; try discriminate.
+  - rewrite whBetaStep_absorbs_mkApp. apply aBeta.
+  - rewrite <- mkApp_goodFn; try not_isApp. apply aAppFn.
+    eapply aCasen; eassumption.
+  - unfold whFixStep in H. case_eq (dnthBody m dts); intros; rewrite H0 in H.
+    + apply aFix. injection H. intros.
+      rewrite <- H1. rewrite pre_whFixStep_absorbs_mkApp. 
+      simpl. unfold whFixStep. rewrite H0. reflexivity. 
+    + discriminate.
+  - rewrite mkApp_idempotent. simpl. rewrite <- (mkApp_goodFn _ _ H3).
+    apply IHawndEval; assumption.
+  - apply aAppArgs. apply awndEval_tappendl. assumption.
+  - rewrite <- mkApp_goodFn; try not_isApp.
+    rewrite <- mkApp_goodFn; try not_isApp. eapply aAppFn. 
+    eapply aProdTy. assumption.
+  - rewrite <- mkApp_goodFn; try not_isApp.
+    rewrite <- mkApp_goodFn; try not_isApp. eapply aAppFn. 
+    eapply aLamTy. assumption.
+  - rewrite <- mkApp_goodFn; try not_isApp.
+    rewrite <- mkApp_goodFn; try not_isApp. eapply aAppFn. 
+    eapply aLetInTy. assumption.
+  - rewrite <- mkApp_goodFn; try not_isApp.
+    rewrite <- mkApp_goodFn; try not_isApp. eapply aAppFn. 
+    eapply aLetInDef. assumption.
+  - rewrite <- mkApp_goodFn; try not_isApp.
+    rewrite <- mkApp_goodFn; try not_isApp. eapply aAppFn. 
+    eapply aCaseTy. assumption.
+  - rewrite <- mkApp_goodFn; try not_isApp.
+    rewrite <- mkApp_goodFn; try not_isApp. eapply aAppFn. 
+    eapply aCaseArg. assumption.
+  - rewrite <- mkApp_goodFn; try not_isApp.
+    rewrite <- mkApp_goodFn; try not_isApp. eapply aAppFn. 
+    eapply aCaseBrs. assumption.
+Qed.
+
+Lemma WFapp_mkApp_WFapp:
+  forall u, WFapp u -> forall t ts, u = mkApp t ts -> WFapp t /\ WFapps ts.
+Proof.
+  induction 1; intros tx tsx h; destruct tx; destruct tsx; simpl in *; 
+  try discriminate; intuition; injection h; intros; subst;
+  try (constructor; assumption); try assumption.
+  - constructor; try assumption. eapply WFapps_tappendl. eassumption.
+  - constructor; try assumption. eapply WFapps_tappendl. eassumption.
+  - eapply WFapps_tappendr. eassumption.
+Qed.
+
+
+Lemma wndEval_awndEval:
+  forall p, WFaEnv p -> 
+  (forall t s, wndEval p t s -> WFapp t -> awndEval p t s) /\
+  (forall ts ss, wndEvals p ts ss -> WFapps ts -> awndEvals p ts ss).
+Proof. 
+  intros p hp. apply wndEvalEvals_ind; intros; try (constructor; assumption);
+               try (inversion H0; subst; constructor; apply H; assumption).
+  - inversion H. subst. eapply aCasen; eassumption.
+  - destruct (WFapp_mkApp_WFapp H0 _ _ eq_refl).
+    apply awndEval_mkApp_mkApp; try assumption.
+    + apply H; assumption.
+Qed.
+
+Lemma awndEval_wndEval:
+  forall p, WFaEnv p -> 
+  (forall t s, awndEval p t s -> WFapp t -> wndEval p t s) /\
+  (forall ts ss, awndEvals p ts ss -> WFapps ts -> wndEvals p ts ss).
+Proof. 
+  intros p hp. apply awndEvalEvals_ind; intros; try (constructor; assumption);
+              try (inversion H0; subst; constructor; apply H; assumption).
+  - inversion H. subst. eapply sCasen; eassumption.
+  - inversion H0. subst. rewrite <- (mkApp_goodFn _ _ H4). apply sAppFn.
+    apply H. assumption.
+Qed.
+
+(** Here is the reason for this alternative definition of wndEval **)
+Lemma awndEval_App_inv:
+  forall p t u, awndEval p t u ->
+  forall fn arg args, t = mkApp fn (tcons arg args) ->
+                      ~ isApp fn -> WFapp t -> WFaEnv p ->
+    (exists nm ty bod, fn = TLambda nm ty bod) \/
+    (exists ds m, fn = TFix ds m) \/
+    (exists fn', wndEval p fn fn') \/
+    (exists arg', wndEval p arg arg') \/
+    (exists args', wndEvals p args args').
+Proof.
+  induction 1; intros;
+  try (rewrite (mkApp_goodFn _ _ H1) in H0; try discriminate);
+  try (rewrite (mkApp_goodFn _ _ H0) in H; try discriminate);
+  try (rewrite (mkApp_goodFn _ _ H2) in H1; try discriminate).
+  - left. exists nm, ty, bod. injection H. intros. subst. reflexivity.
+  - right. left. exists dts, m. injection H0. intros. subst. reflexivity.
+  - right. right. left. injection H0. intros. subst.
+    exists r. inversion H2. apply awndEval_wndEval; assumption.
+  - right. right. right. left. injection H0. intros. subst.
+    exists brg. inversion H2. apply awndEval_wndEval; assumption.
+  - right. right. right. right. inversion H2. injection H0. intros. subst.
+    exists brgs. apply awndEval_wndEval; assumption.
+Qed.
+
+(***
+Lemma wndEval_pres_WFapp:
+  forall p, WFaEnv p -> 
+  (forall t s, wndEval p t s -> WFapp t -> WFapp s) /\
+  (forall ts ss, wndEvals p ts ss -> WFapps ts -> WFapps ss).
+Proof.
+  intros p hp.
+  apply wndEvalEvals_ind; intros;
+  try (solve [inversion_Clear H0; constructor; intuition]).
+  - assert (j:= Lookup_pres_WFapp hp l). inversion j. intuition.
+  - inversion_Clear H. inversion_Clear H4.
+    apply whBetaStep_pres_WFapp; assumption.
+  - inversion_Clear H. apply instantiate_pres_WFapp; assumption.
+  - inversion_Clear H. eapply (whCaseStep_pres_WFapp H5). eapply wfanil.
+    eassumption.
+  - inversion_Clear H. inversion_Clear H3. unfold whCaseStep in e0.
+    assert (j:= tnth_pres_WFapp H5 n). destruct (tnth n brs).
+    + injection e0. intros. rewrite <- H. apply mkApp_pres_WFapp.
+      * eapply (tskipn_pres_WFapp). apply wfacons. apply H7. apply H8. apply e.
+      * apply j. reflexivity.
+    + discriminate.
+  - inversion_Clear H. inversion_Clear H4. unfold whFixStep in e.
+    assert (j:= dnthBody_pres_WFapp H0 m). destruct (dnthBody m dts).
+    injection e. intros. rewrite <- H. apply mkApp_pres_WFapp.
+    + apply wfacons; assumption.
+    + apply fold_left_pres_WFapp. intros.
+      * { apply instantiate_pres_WFapp. 
+          - assumption.
+          - auto. }
+      * eapply j. reflexivity.
+    + discriminate.
+  - inversion_Clear H. assumption.
+  - destruct (WFapp_mkApp_WFapp H0 _ _ eq_refl). inversion_Clear H2.
+    apply mkApp_pres_WFapp.
+    + constructor; assumption.
+    + intuition.
+Qed.
+
+Lemma wndEval_tappendl:
+  forall p bs cs, wndEvals p bs cs ->
+  forall ds, wndEvals p (tappend bs ds) (tappend cs ds).
+Proof.
+  induction 1; intros.
+  - constructor. assumption.
+  - simpl. apply saTl. apply IHwndEvals.
+Qed.
+
+Lemma wndEval_tappendr:
+  forall p bs cs, wndEvals p bs cs ->
+  forall ds, wndEvals p (tappend ds bs) (tappend ds cs).
+Proof.
+  intros p bs cs h ds. induction ds; simpl.
+  - assumption.
+  - apply saTl. apply IHds.
+Qed.
+
+(***
+Lemma wndEval_pres_Crct:
+  forall p,
+  (forall t s, wndEval p t s -> forall n, Crct p n t -> Crct p n s) /\
+  (forall ts ss, wndEvals p ts ss ->
+                   forall n, Crcts p n ts -> Crcts p n ss).
+Proof.
+  intros p. apply wndEvalEvals_ind; intros.
+  - eapply LookupDfn_pres_Crct; try eassumption.
+  - destruct (Crct_invrt_App H eq_refl) as [h1 [h2 [h3 h4]]].
+    destruct (Crct_invrt_Lam h1 eq_refl). 
+    unfold whBetaStep. apply mkApp_pres_Crct; try assumption. 
+    apply instantiate_pres_Crct; try assumption.
+    omega.
+  - destruct (Crct_invrt_LetIn H eq_refl) as [h1 [h2 h3]].
+    apply instantiate_pres_Crct; try assumption. omega.
+  - destruct (Crct_invrt_Case H eq_refl) as [h1 [h2 h3]].
+    refine (whCaseStep_pres_Crct _ _ _ e); trivial.
+    + apply CrctsNil. eapply Crct_Sort. eassumption.
+  - destruct (Crct_invrt_Case H eq_refl) as [h1 [h2 h3]].
+    refine (whCaseStep_pres_Crct _ _ _ e0); trivial.
+    + apply (tskipn_pres_Crct _ e).
+      * destruct (Crct_invrt_App h2 eq_refl) as [j1 [j2 [j3 j4]]].
+        apply CrctsCons; assumption.
+  - destruct (Crct_invrt_App H eq_refl) as [h1 [h2 [h3 h4]]].
+    assert (j:= @Crct_invrt_Fix _ _ _ h1 dts m eq_refl).
+    refine (whFixStep_pres_Crct _ _ _ e); try assumption.
+    + constructor; assumption. 
+  - destruct (Crct_invrt_Cast H eq_refl) as [h1 h2]. assumption.
+  - destruct (Crct_invrt_App H0 eq_refl) as [h1 [h2 [h3 h4]]].
+    apply mkApp_pres_Crct.
+    + apply H. assumption.
+    + apply CrctsCons; assumption.
+  - destruct (Crct_invrt_App H0 eq_refl) as [h1 [h2 [h3 h4]]].
+    apply CrctApp; intuition. 
+  - destruct (Crct_invrt_App H0 eq_refl) as [h1 [h2 [h3 h4]]].
+    apply CrctApp; intuition.
+  - destruct (Crct_invrt_Prod H0 eq_refl) as [h1 h2].
+    apply CrctProd; try assumption.
+    + apply H; assumption.
+  - destruct (Crct_invrt_Lam H0 eq_refl) as [h1 h2].
+    apply CrctLam; try assumption.
+    + apply H; assumption.
+  - destruct (Crct_invrt_LetIn H0 eq_refl) as [h1 [h2 h3]].
+    apply CrctLetIn; try assumption.
+    + apply H; assumption.
+  - destruct (Crct_invrt_LetIn H0 eq_refl) as [h1 [h2 h3]].
+    apply CrctLetIn; try assumption.
+    + apply H; assumption.
+  - destruct (Crct_invrt_Case H0 eq_refl) as [h1 [h2 h3]].
+    apply CrctCase; try assumption.
+    + apply H; assumption.
+  - destruct (Crct_invrt_Case H0 eq_refl) as [h1 [h2 h3]].
+    apply CrctCase; try assumption.
+    + apply H; assumption.
+  - destruct (Crct_invrt_Case H0 eq_refl) as [h1 [h2 h3]].
+    apply CrctCase; try assumption.
+    + apply H; assumption.
+  - inversion_Clear H0. apply CrctsCons; try assumption.
+    apply H. assumption.
+  - inversion_Clear H0. apply CrctsCons; try assumption.
+    apply H. assumption.
+Qed.
+***)
+
+(** reduction preserves WFTrm **
+Goal forall p t s, wndEval p t s -> forall n, WFTrm t n -> WFTrm s n.
+Proof.
+  induction 1; intros nx h. try (solve [apply wfa1; not_isApp]);
+  try (solve [apply mkApp_WFApp]);
+  try (solve [eapply whCaseStep_WFApp; eassumption]);
+  try (solve [apply wfa2; assumption]).
+- apply inst_WFApp.
+- eapply whFixStep_WFApp. eassumption.
+Qed.
+**)
+
+Lemma wndEval_Lam_inv:
+  forall p nm tp bod s,
+    wndEval p (TLambda nm tp bod) s ->
+    exists tp', wndEval p tp tp' /\ s = (TLambda nm tp' bod).
+intros p nm tp bod s h. inversion_Clear h.
+- assert (j:= mkApp_isApp t arg args).
+  destruct j as [x0 [x1 [x2 k]]]. rewrite k in H. discriminate.
+- exists t2. split; [assumption | reflexivity].
+Qed.
+
+
+(** when reduction stops **)
+Definition no_wnd_step (p:environ) (t:Term) : Prop :=
+  no_step (wndEval p) t.
+Definition no_wnds_step (p:environ) (ts:Terms) : Prop :=
+  no_step (wndEvals p) ts.
+
+
+(** reflexive-transitive closure of wndEval **)
+Inductive wndEvalRTC (p:environ): Term -> Term -> Prop :=
+(** | wERTCrfl: forall t, WNorm t -> wndEvalRTC p t t ??? **)
+| wERTCrfl: forall t, wndEvalRTC p t t
+| wERTCstep: forall t s, wndEval p t s -> wndEvalRTC p t s
+| wERTCtrn: forall t s u, wndEvalRTC p t s -> wndEvalRTC p s u ->
+                          wndEvalRTC p t u.
+Inductive wndEvalsRTC (p:environ): Terms -> Terms -> Prop :=
+(** | wEsRTCrfl: forall ts, WNorms ts -> wndEvalsRTC p ts ts ??? **)
+| wEsRTCrfl: forall ts, wndEvalsRTC p ts ts
+| wEsRTCstep: forall ts ss, wndEvals p ts ss -> wndEvalsRTC p ts ss
+| wEsRTCtrn: forall ts ss us, wndEvalsRTC p ts ss -> wndEvalsRTC p ss us ->
+                          wndEvalsRTC p ts us.
+Hint Constructors wndEvalRTC wndEvalsRTC.
+
+Lemma wndEvalRTC_pres_WFapp:
+  forall p t s, wndEvalRTC p t s -> WFaEnv p -> WFapp t -> WFapp s.
+Proof.
+  induction 1; intros; try assumption.
+  - eapply (proj1 (wndEval_pres_WFapp H0)); eassumption.
+  - apply IHwndEvalRTC2; try assumption.
+    + apply IHwndEvalRTC1; assumption.
+Qed.
+
+
+(** transitive closure of wndEval **)
+(***
+Definition wndEvalTC (p:environ) := clos_trans Term (wndEval p).
+Definition wndEvalTC1n (p:environ) := clos_trans_1n Term (wndEval p).
+Definition wndEvalTCn1 (p:environ) := clos_trans_n1 Term (wndEval p).
+Hint Constructors clos_trans clos_trans_1n clos_trans_n1.
+Notation wETCstep := (t_step).
+Notation wETCtrn := (t_trans).
+****)
+Inductive wndEvalTC (p:environ): Term -> Term -> Prop :=
+| wETCstep: forall t s, wndEval p t s -> wndEvalTC p t s
+| wETCtrn: forall t s, wndEvalTC p t s -> forall u, wndEvalTC p s u ->
+                          wndEvalTC p t u.
+Inductive wndEvalsTC (p:environ): Terms -> Terms -> Prop :=
+| wEsTCstep: forall ts ss, wndEvals p ts ss -> wndEvalsTC p ts ss
+| wEsTCtrn: forall ts ss, wndEvalsTC p ts ss -> forall us, wndEvalsTC p ss us ->
+                          wndEvalsTC p ts us.
+Hint Constructors wndEvalTC wndEvalsTC.
+
+Lemma wndEvalTC_pres_WFapp:
+  forall p t s, wndEvalTC p t s -> WFaEnv p -> WFapp t -> WFapp s.
+Proof.
+  induction 1; intros.
+  - eapply (proj1 (wndEval_pres_WFapp H0)); eassumption.
+  - apply IHwndEvalTC2; try assumption.
+    + apply IHwndEvalTC1; assumption.
+Qed.
+
+Inductive wndEvalTCl (p:environ): Term -> Term -> Prop :=
+| wETClstep: forall t s, wndEval p t s -> wndEvalTCl p t s
+| wETCltrn: forall t s, wndEvalTCl p t s -> forall u, wndEval p s u ->
+                          wndEvalTCl p t u.
+Inductive wndEvalsTCl (p:environ): Terms -> Terms -> Prop :=
+| wEsTClstep: forall ts ss, wndEvals p ts ss -> wndEvalsTCl p ts ss
+| wEsTCltrn: forall ts ss, wndEvalsTCl p ts ss -> 
+                           forall us, wndEvals p ss us ->
+                          wndEvalsTCl p ts us.
+Hint Constructors wndEvalTCl wndEvalsTCl.
+
+Axiom wndEvalTC_wndEvalTCl:
+  forall p t s, wndEvalTC p t s -> wndEvalTCl p t s.
+Axiom wndEvalTl_wndEvalTC:
+  forall p t s, wndEvalTCl p t s -> wndEvalTC p t s.
+
+
+(** transitive congruence rules **)
+(***
+Lemma wndEvalRTC_App_fn:
+  forall p fn fn' a1 args,
+    wndEvalRTC p fn fn' -> ~ (isLambda fn') -> ~ (isFix fn') -> 
+      wndEvalRTC p (TApp fn a1 args) (TApp fn' a1 args).
+induction 1; intros.
+- eapply (@wERTCtrn _ _ (TApp t a1 args)). apply wERTCrfl. apply WNApp; auto. inversion H.
+- constructor. apply sAppFn. assumption.
+- eapply wERTCtrn. apply IHwndEvalRTC1. apply IHwndEvalRTC2.
+Qed.
+***)
+
+
+(***
+Lemma wndEvalRTC_App_fn:
+  forall p fn fn',
+    wndEvalRTC p fn fn' -> 
+    forall  a1 args,
+      wndEvalRTC p (mkApp fn (tcons a1 args)) (mkApp fn' (tcons a1 args)).
+induction 1; intros.
+- apply wERTCrfl.
+- constructor. apply sAppFn. assumption.
+- eapply wERTCtrn. 
+  + apply IHwndEvalRTC1.
+  + apply IHwndEvalRTC2.
+Qed.
+***)
+
+(**
+Lemma wndEval_App_fn:
+  forall p fn fn', wndEval p fn fn' ->
+    forall a1 args, WFapp (TApp fn a1 args) ->
+    (~ isApp fn' /\ wndEval p (TApp fn a1 args) (TApp fn' a1 args)) \/
+    (isApp fn' /\ wndEval p (TApp fn a1 args) (mkApp fn' (tcons a1 args))). 
+Proof.
+  induction 1; simpl; intros h; intros.
+  - destruct (isApp_dec t) as [j0 | j0].
+    + right. intuition. 
+    + left. rewrite <- (mkApp_goodFn _ _ j0). intuition. 
+  - inversion_clear H. elim H0. exists (TLambda nm ty bod), arg, args. 
+    reflexivity.
+  - inversion_Clear H. destruct (isApp_dec (instantiate dfn 0 bod)). 
+    + right. destruct i as [x0 [x1 [x2 j1]]]. intuition. 
+      rewrite j1. intuition. 
+    + left. rewrite <- (mkApp_goodFn _ _ n). intuition. 
+  - inversion_Clear H0. destruct (isApp_dec s).
+    + right. intuition. 
+    + left. intuition. rewrite <- (mkApp_goodFn _ _ n0). apply sAppFn.
+      apply sCase0. assumption.
+  - inversion_Clear H1. destruct (isApp_dec s).
+    + right. intuition. apply sAppFn. eapply sCasen; eassumption. 
+    + left. intuition. rewrite <- (mkApp_goodFn _ _ n0). apply sAppFn. 
+      eapply sCasen; eassumption.
+  - inversion_clear H0. elim H1. exists (TFix dts m), arg, args. reflexivity.
+  - inversion_Clear H. destruct (isApp_dec t).
+    + right. intuition. 
+    + left. rewrite <- (mkApp_goodFn _ _ n). intuition. 
+  - inversion_clear H0. elim H1. exists t, arg, args. reflexivity.
+  - inversion_clear H0. elim H1. exists t, arg, args. reflexivity.
+  - inversion_clear H0. elim H1. exists t, arg, args. reflexivity.
+  - left. rewrite <- (@mkApp_goodFn (TProd nm t2 bod)).
+    + intuition. destruct H1 as [x0 [x1 [x2 j]]]. discriminate.
+    + not_isApp.
+  - left. rewrite <- (@mkApp_goodFn (TLambda nm t2 bod)).
+    + intuition. destruct H1 as [x0 [x1 [x2 j]]]. discriminate.
+    + not_isApp.
+  - left. rewrite <- (@mkApp_goodFn (TLetIn nm d t2 bod)).
+    + intuition. destruct H1 as [x0 [x1 [x2 j]]]. discriminate.
+    + not_isApp.
+  - left. rewrite <- (@mkApp_goodFn (TLetIn nm d2 t bod)).
+    + intuition. destruct H1 as [x0 [x1 [x2 j]]]. discriminate.
+    + not_isApp.
+  - left. rewrite <- (@mkApp_goodFn (TCase np uy mch brs)).
+    + intuition. destruct H1 as [x0 [x1 [x2 j]]]. discriminate.
+    + not_isApp.
+  - left. rewrite <- (@mkApp_goodFn (TCase np ty can brs)).
+    + intuition.  destruct H1 as [x0 [x1 [x2 j]]]. discriminate.
+    + not_isApp.
+  - left. rewrite <- (@mkApp_goodFn (TCase np ty mch brs')).
+    + intuition.  destruct H1 as [x0 [x1 [x2 j]]]. discriminate.
+    + not_isApp.
+Qed.
+
+
+(**
+Lemma wndEval_App_fn_cor:
+  forall p fn fn', wndEval p fn fn' ->
+    forall a1 args, WFapp (TApp fn a1 args) ->
+      wndEval p (TApp fn a1 args) (mkApp fn' (tcons a1 args)).
+Proof.
+  intros p fn fn' h1 a1 args h2. 
+  destruct (isApp_dec fn'); destruct (wndEval_App_fn h1 h2).
+***)
+
+
+Lemma wndEvalTC_App_fn:
+  forall p fn fn', wndEval p fn fn' ->
+    forall a1 args, WFapp (TApp fn a1 args) ->
+    (~ isApp fn' /\ wndEvalTC p (TApp fn a1 args) (TApp fn' a1 args)) \/
+    (isApp fn' /\ wndEvalTC p (TApp fn a1 args) (mkApp fn' (tcons a1 args))).
+Proof.
+  intros. destruct (wndEval_App_fn H H0). 
+  - left. intuition.
+  - right. intuition.
+Qed.
+***)
+
+Lemma wndEval_mkApp_mkApp:
+  forall p s u, wndEval p s u ->
+  forall a1 args,
+     wndEval p (mkApp s (tcons a1 args)) (mkApp u (tcons a1 args)).
+Proof.
+  induction 1; simpl; intros; auto; try discriminate.
+  - rewrite <- mkApp_goodFn; try not_isApp. apply sAppFn.
+    apply sConst. assumption.
+  - rewrite whBetaStep_absorbs_mkApp. apply sBeta.
+  - rewrite <- mkApp_goodFn; try not_isApp. apply sAppFn.
+    apply sLetIn.
+  - rewrite <- mkApp_goodFn; try not_isApp. apply sAppFn.
+    apply sCase0. assumption.
+  - rewrite <- mkApp_goodFn; try not_isApp. apply sAppFn.
+    eapply sCasen; eassumption.
+  - unfold whFixStep in H. case_eq (dnthBody m dts); intros; rewrite H0 in H.
+    + apply sFix. injection H. intros.
+      rewrite <- H1. rewrite pre_whFixStep_absorbs_mkApp. 
+      simpl. unfold whFixStep. rewrite H0. reflexivity. 
+    + discriminate.
+  - rewrite <- mkApp_goodFn; try not_isApp. apply sAppFn.
+    eapply sCast; eassumption.
+  - eapply sAppArgs. eapply wndEval_tappendl. assumption.
+  - rewrite <- mkApp_goodFn; try not_isApp.
+    rewrite <- mkApp_goodFn; try not_isApp. eapply sAppFn. 
+    eapply sProdTy. assumption.
+  - rewrite <- mkApp_goodFn; try not_isApp.
+    rewrite <- mkApp_goodFn; try not_isApp. eapply sAppFn. 
+    eapply sLamTy. assumption.
+  - rewrite <- mkApp_goodFn; try not_isApp.
+    rewrite <- mkApp_goodFn; try not_isApp. eapply sAppFn. 
+    eapply sLetInTy. assumption.
+  - rewrite <- mkApp_goodFn; try not_isApp.
+    rewrite <- mkApp_goodFn; try not_isApp. eapply sAppFn. 
+    eapply sLetInDef. assumption.
+  - rewrite <- mkApp_goodFn; try not_isApp.
+    rewrite <- mkApp_goodFn; try not_isApp. eapply sAppFn. 
+    eapply sCaseTy. assumption.
+  - rewrite <- mkApp_goodFn; try not_isApp.
+    rewrite <- mkApp_goodFn; try not_isApp. eapply sAppFn. 
+    eapply sCaseArg. assumption.
+  - rewrite <- mkApp_goodFn; try not_isApp.
+    rewrite <- mkApp_goodFn; try not_isApp. eapply sAppFn. 
+    eapply sCaseBrs. assumption.
+Qed.
+
+
+(**
+(****  HERE is the problem  ******)
+Goal
+  forall p s u, wndEval p s u ->
+  forall fs bs bss, s = TApp fs bs bss -> ~ isApp u ->
+  forall a1 args,
+     wndEval p (mkApp s (tcons a1 args)) (TApp u a1 args).
+Proof.
+  induction 1; simpl; intros; auto; try discriminate.
+  - destruct (not_isApp_whBetaStep _ _ _ H0). subst. simpl.
+    injection H. intros. subst. clear H. 
+  - rewrite whBetaStep_absorbs_mkApp. apply sBeta.
+  - unfold whFixStep in H. case_eq (dnthBody m dts); intros; rewrite H2 in H.
+    + apply sFix. injection H. intros.
+      rewrite <- H3. rewrite pre_whFixStep_absorbs_mkApp. 
+      simpl. unfold whFixStep. rewrite H2. reflexivity. 
+    + discriminate.
+  - rewrite mkApp_idempotent. apply sAppFn. assumption.
+  - injection H0. intros. subst. clear H0.
+    injection H1. intros. subst. clear H1. apply sAppArgs.
+    apply wndEval_tappendl. assumption.
+Qed.
+***)
+
+(****  HERE is the problem  ******
+Lemma wndEvalTC_App_fn':
+  forall p fn fn', wndEvalTC p fn fn' -> WFaEnv p ->
+  forall a1 args, WFapp (TApp fn a1 args) ->
+    (~ isApp fn' /\ wndEvalTC p (TApp fn a1 args) (TApp fn' a1 args)) \/
+    (isApp fn' /\ wndEvalTC p (TApp fn a1 args) (mkApp fn' (tcons a1 args))).
+Proof.
+  induction 1; intros.
+  - destruct (wndEvalTC_App_fn H H1) as [[j1 j2]|[j1 j2]].
+    + left. intuition.
+    + right. intuition.
+  - inversion H2. subst.
+
+    destruct (IHwndEvalTC1 H1 _ _ H2) as [[j1 j2]|[j1 j2]].
+    assert (j: WFapp (TApp s a1 args)).
+    { constructor; try assumption.
+      eapply wndEvalTC_pres_WFapp; eassumption. }
+    destruct (IHwndEvalTC2 H1 _ _ j) as [[k1 k2]|[k1 k2]].
+    + left. intuition. eapply wETCtrn; eassumption.
+    + right. intuition. eapply wETCtrn; eassumption.
+    +  Check (IHwndEvalTC2 H1). as [[k1 k2]|[k1 k2]].
+
+
+
+  - destruct (isApp_dec s) as [hs|hs].
+    + right. intuition.
+    + left. intuition.
+      rewrite <- (@mkApp_goodFn s). apply wETClstep. apply sAppFn. assumption.
+      assumption.
+  - destruct (isApp_dec u) as [hu|hu].
+    + right. intuition. destruct (H3 _ _ H2) as [[j1 j2]|[j1 j2]].
+    + left. intuition.
+
+destruct (IHwndEvalTCl H1 _ _ H2); destruct H3.
+    + contradiction.
+    + destruct (isApp_dec u) as [hu|hu]. 
+      * right. intuition. eapply wETCltrn. eapply H4.
+        destruct hs as [s0 [s1 [s2 js]]].
+        destruct hu as [u0 [u1 [u2 ju]]].
+        eapply wndEval_mkApp_mkApp; eassumption.
+      * left. intuition. inversion H2. subst. eapply wETCltrn. eassumption.
+        destruct hs as [s0 [s1 [s2 js]]]. rewrite js. simpl.
+        rewrite js in H0. rewrite js in H.
+
+
+        rewrite (@mkApp_goodFn s).
+
+Check (wndEvalTC_App_fn).
+
+Lemma wndEvalTC_App_fn':
+  forall p fn fn', wndEvalTCl p fn fn' -> WFaEnv p ->
+  forall a1 args, WFapp (TApp fn a1 args) ->
+    (~ isApp fn' /\ wndEvalTCl p (TApp fn a1 args) (TApp fn' a1 args)) \/
+    (isApp fn' /\ wndEvalTCl p (TApp fn a1 args) (mkApp fn' (tcons a1 args))).
+Proof.
+  induction 1; intros. destruct (isApp_dec s) as [hs|hs]. 
+  - right. intuition.
+  - left. intuition.
+    rewrite <- (@mkApp_goodFn s). apply wETClstep. apply sAppFn. assumption.
+    assumption.
+  - destruct (IHwndEvalTCl H1 _ _ H2).
+    + destruct H3. contradiction.
+    + destruct H3. destruct (isApp_dec u) as [hu|hu]. 
+      * right. intuition. eapply wETCltrn. eapply H4.
+        eapply wndeval_mkApp_mkApp. assumption.
+
+
+  destruct hs as [s0 [s1 [s2 js]]].
+  - right. exists s0, s1, s2. intuition.
+  - left. destruct (wndEvalTC_App_fn H H1). assumption.
+    + rewrite <- (@mkApp_goodFn s). apply wETCstep. apply sAppFn. assumption.
+      assumption.
+  - destruct (IHwndEvalTC1 H1 _ _ H2) as [k|k].
+
+
+Lemma wndEvalTC_App_fn':
+  forall p fn fn', wndEvalTC p fn fn' -> WFaEnv p ->
+  forall a1 args, WFapp (TApp fn a1 args) ->
+    (~ isApp fn' /\ wndEvalTC p (TApp fn a1 args) (TApp fn' a1 args)) \/
+    (isApp fn' /\ wndEvalTC p (TApp fn a1 args) (mkApp fn' (tcons a1 args))).
+Proof.
+  induction 1; intros; destruct (isApp_dec s) as [hs|hs]. 
+  - right. intuition.
+  - left. intuition.
+    rewrite <- (@mkApp_goodFn s). apply wETCstep. apply sAppFn. assumption.
+    assumption.
+  - destruct (IHwndEvalTC1 H1 _ _ H2).
+    + destruct H3. contradiction.
+    + destruct H3.
+
+
+  destruct hs as [s0 [s1 [s2 js]]].
+  - right. exists s0, s1, s2. intuition.
+  - left. destruct (wndEvalTC_App_fn H H1). assumption.
+    + rewrite <- (@mkApp_goodFn s). apply wETCstep. apply sAppFn. assumption.
+      assumption.
+  - destruct (IHwndEvalTC1 H1 _ _ H2) as [k|k].
+
+
+
+
+
+Proof.
+  induction 1; intros;
+  destruct (isApp_dec s) as [hs|hs]. destruct hs as [s0 [s1 [s2 js]]].
+  - right. exists s0, s1, s2. intuition.
+  - left. destruct (wndEvalTC_App_fn H H1). assumption.
+    + rewrite <- (@mkApp_goodFn s). apply wETCstep. apply sAppFn. assumption.
+      assumption.
+  - destruct hs as [s0 [s1 [s2 js]]].
+    destruct (isApp_dec u) as [hu|hu]. destruct hu as [u0 [u1 [u2 ju]]].
+    + right. exists u0, u1, u2. split. assumption.
+      * { eapply wETCtrn. destruct (IHwndEvalTC1 H1 _ _ H2) as [k|k]. 
+          - rewrite js in k.  
+            assert (l:WFapp (TApp (TApp s0 s1 s2) a1 args)).
+            { eapply wndEvalTC_pres_WFapp; eassumption. }
+            inversion_Clear l. eassumption.
+          -
+
+subst. eassumption.
+          -
+
+  intros p fn fn' h1 hp a1 args h4.
+  induction h1; intros;
+  destruct (isApp_dec s) as [hs|hs]. destruct hs as [s0 [s1 [s2 js]]].
+  - right. exists s0, s1, s2. intuition.
+  - left. assert (j:= wndEvalTC_App_fn H h4).
+    rewrite mkApp_goodFn in j; try assumption.
+    + inversion_Clear h4. left. rewrite <- (@mkApp_goodFn s). 
+      apply sAppFn. assumption. assumption.
+  - destruct hs as [s0 [s1 [s2 js]]].
+    destruct (isApp_dec u) as [hu|hu]. destruct hu as [u0 [u1 [u2 ju]]].
+    + right. exists u0, u1, u2. split. assumption.
+      * { eapply wETCtrn. destruct (IHh1_1 h4) as [k|k]. 
+          - eassumption.
+          - subst.
+
+  - destruct (isApp_dec u).
+    + right. destruct i0 as [x0 [x1 [x2 j]]]. exists x0, x1, x2. split.
+      * assumption.
+      * { destruct (IHh1_1 h4) as [j0 | j0]. 
+          - assert (j1:= wndEvalTC_pres_WFapp j0 hp h4). inversion_Clear j1.
+            contradiction.
+          - destruct j0 as [y0 [y1 [y2 j1]]]. destruct j1 as [j2 j3].
+            eapply wETCtrn.
+            + eassumption.
+            + subst. simpl.
+            simpl in IHh1_2. simpl in IHh1_2.
+Check (IHh1_1 h4).
+
+eapply wETCtrn. apply (IHh1_1 h4).
+
+
+ destruct (IHh1_1 h4) as [j0 | j0].
+    + assert (j1:= wndEvalTC_pres_WFapp j0 hp h4). inversion_Clear j1.
+      contradiction.
+    + destruct j0 as [x0 [x1 [x2 j]]]; destruct (isApp_dec u). 
+
+
+
+right. exists x0, x1, x2.
+      destruct j as [j1 j2].
+
+
+
+  - right. destruct i as [x0 [x1 [x2 j]]]. exists x0, x1, x2. intuition.
+  - inversion h4. subst. eapply wETCtrn.
+
+Check (proj1 (wndEval_pres_WFapp hp) _ _ H).
+  - inversion h4. subst. eapply wETCtrn.
+    + inversion_Clear h1_1. 
+      * apply wETCstep. apply sAppFn. eassumption.
+      *
+    + apply IHh1_1. apply wndEvalTC_preserves_WFapp. assumption.
+
+
+
+    + apply wndEval_App_fn; eassumption.
+    + assert (j:= proj1 (wndEval_pres_WFapp _) _ _ (sAppFn _ _ h1)).
+    + destructj:=  (isApp_dec s).
+      * destruct i as [x0 [x1 [x2 j]]]. rewrite j. simpl.
+
+
+Lemma wndEvalTC_App_fn':
+  forall p fn fn', wndEvalTC p fn fn' -> WFaEnv p ->
+    forall a1 args, WFapp (TApp fn a1 args) ->
+      wndEvalTC p (mkApp fn (tcons a1 args)) (mkApp fn' (tcons a1 args)).
+Proof.
+  Check (mkApp_goodFn).
+  induction 1; intros.
+  - apply wndEvalTC_App_fn. 
+    + assumption.
+    + assumption.
+  - eapply wETCtrn.
+    + apply wndEval_App_fn; eassumption.
+    + assert (j:= proj1 (wndEval_pres_WFapp H1) _ _ (sAppFn _ _ H) H2).
+    + destructj:=  (isApp_dec s).
+      * destruct i as [x0 [x1 [x2 j]]]. rewrite j. simpl.
+
+
+    + Check (wndEval_App_fn).
+
+    + inversion_Clear H.
+      * apply wndEval_App_fn; eassumption.
+      * apply IHwndEvalTC1; assumption.
+    + destruct (isApp_dec s).
+      * destruct i as [x0 [x1 [x2 j]]]. rewrite j. simpl.
+
+
+      *    + inversion H. apply wndEvalTC_App_fn. apply H3. assumption.
+      apply IHwndEvalTC1. assumption. assumption.
+
+    + inversion_Clear H2. assert (j:= wndEvalTC_preserves_WFapp H H1 H7).
+      rewrite mkApp_goodFn. apply IHwndEvalTC2. assumption.
+      constructor; try assumption.
+Qed.
+*******)
+
+(****  HERE is the problem  ******
+Lemma wndEvalTC_App_fn:
+  forall p fn fn', wndEvalTC p fn fn' -> WFaEnv p ->
+    forall a1 args, WFapp (TApp fn a1 args) ->
+      wndEvalTC p (TApp fn a1 args) (mkApp fn' (tcons a1 args)).
+Proof.
+  induction 1; intros.
+  - apply wndEvalTC_App_fn'.
+    + assumption.
+    + assumption.
+  - eapply wETCtrn.
+    + apply IHwndEvalTC1; assumption.
+    + inversion_Clear H2. assert (j:= wndEvalTC_preserves_WFapp H H1 H7).
+      rewrite mkApp_goodFn. apply IHwndEvalTC2. assumption.
+      constructor; try assumption.
+Qed.
+*******)
+
+(****
+Lemma wndEvalTC_App_fn:
+  forall p fn fn', wndEval p fn fn' ->
+    forall a1 args, 
+      wndEvalTC p (mkApp fn (tcons a1 args)) (mkApp fn' (tcons a1 args)).
+Proof.
+  induction 1; simpl; intros h; intros.
+  - apply wETCstep. apply sAppFn; constructor. trivial.
+  - apply wETCstep. unfold whBetaStep.
+    rewrite mkApp_idempotent. apply sBeta.
+  - apply wETCstep. apply sAppFn. apply sLetIn.
+  - apply wETCstep. apply sAppFn. apply sCase0. assumption.
+  - apply wETCstep. apply sAppFn. eapply sCasen; eassumption.
+  - unfold whFixStep in H.
+    case_eq (dnthBody m dts); intros; rewrite H0 in H.
+    + injection H. intros. rewrite <- H1.
+      rewrite mkApp_idempotent. apply wETCstep. apply sFix. unfold whFixStep.
+      rewrite H0. reflexivity.
+    + discriminate.
+  - apply wETCstep. apply sAppFn. apply sCast.
+  - apply wETCstep. rewrite mkApp_idempotent. simpl. apply sAppFn.
+
+destruct (dnthBody m dts).
+    + injection H. intros. rewrite <- H0. rewrite mkApp_idempotent.
+      apply wETCstep. apply sFix. unfold whFixStep.
+
+
+Lemma wndEvalTC_App_fn:
+  forall p fn fn', wndEvalTC p fn fn' ->
+   forall a1 args, WFapp (TApp fn a1 args) ->
+    wndEvalTC p (mkApp fn (tcons a1 args)) (mkApp fn' (tcons a1 args)).
+Proof.
+  induction 1; intros. 
+  - rewrite (WFapp_mkApp_TApp H0 eq_refl).
+    constructor. apply sAppFn; trivial.
+  - eapply wETCtrn. 
+    + apply IHwndEvalTC1. assumption.
+    + eapply IHwndEvalTC2. inversion_Clear H1. constructor; try assumption.
+      * 
+
+
+
+Lemma wndEvalTC_App_fn:
+  forall p fn fn', wndEvalTC p fn fn' -> ~ isApp fn' ->
+   forall n a1 args, Crct p n (TApp fn a1 args) ->
+    wndEvalTC p (TApp fn a1 args) (TApp fn' a1 args).
+Proof.
+  unfold wndEvalTC. intros p fn fn1 h0. 
+  assert (j0:= clos_trans_t1n Term (wndEval p) _ _ h0).
+  apply clos_t1n_trans.
+  induction 1; intros.
+  - constructor. apply sAppFn; trivial.
+  - eapply wETCtrn. eapply IHclos_trans1; trivial.
+    + admit.
+
+
+  - eapply wETCtrn. 
+    + eapply wETCstep. apply sAppFn; trivial.
+      *
+    +
+
+  - eapply wETCtrn. apply IHwndEvalTC1; trivial.
+    + admit.
+Qed.
+***)
+
+(*************
+Goal
+  forall fn p fn',
+    wndEvalTC p fn fn' -> ~ isApp fn ->
+    forall  a1 args,
+      wndEvalTC p (TApp fn a1 args) (mkApp fn' (tcons a1 args)).
+Proof.
+  apply (@wf_ind Term TrmSize
+           (fun fn:Term => forall p fn', wndEvalTC p fn fn' -> ~ isApp fn ->
+            forall a1 args, 
+             wndEvalTC p (TApp fn a1 args) (mkApp fn' (tcons a1 args)) )).
+  intros t wih p fn' h1 a1 args h2.
+  induction h1.
+  - constructor. apply sAppFn; assumption.
+  - eapply wETCtrn. apply IHh1_1; trivial.
+*********)
+
+(*************
+apply sAppFn. assumption. inversion H; try (solve [not_isApp]).
+    + destruct H1. unfold isApp. exists t, a1, args. reflexivity.
+    + assumption.
+  - eapply wETCtrn.
+    + apply IHwndEvalTC1. assumption.
+    + assert (j0:= wndEvalTC_WFApp H). 
+      assert (j1:= mkApp_isApp_lem s a1 args).
+      destruct j1. destruct H2. destruct H2. destruct H2 as [k1 [k2 | k3]].
+      * rewrite k1. destruct k2 as [l1 [l2 [l3 l4]]].
+        rewrite l2. rewrite <- l3. rewrite l4. simpl.
+        apply IHwndEvalTC2.
+
+
+
+Lemma wndEvalTC_App_fn:
+  forall fn p fn',
+    wndEvalTC p fn fn' ->
+    forall  a1 args, WFApp (TApp fn a1 args) ->
+      wndEvalTC p (TApp fn a1 args) (mkApp fn' (tcons a1 args)).
+Proof.
+  induction 1; intros.
+  - constructor. apply sAppFn. assumption. inversion H0.
+    + destruct H1. unfold isApp. exists t, a1, args. reflexivity.
+    + assumption.
+  - eapply wETCtrn.
+    + apply IHwndEvalTC1. assumption.
+    + assert (j0:= wndEvalTC_WFApp H). 
+      assert (j1:= mkApp_isApp_lem s a1 args).
+      destruct j1. destruct H2. destruct H2. destruct H2 as [k1 [k2 | k3]].
+      * rewrite k1. destruct k2 as [l1 [l2 [l3 l4]]].
+        rewrite l2. rewrite <- l3. rewrite l4. simpl.
+        apply IHwndEvalTC2.
+
+apply IHwndEvalTC2. assumption.
+
+
+  apply (@wf_ind Term TrmSize
+           (fun fn:Term => forall p fn', wndEvalTC p fn fn' ->
+            forall  a1 args, WFApp (TApp fn a1 args) ->
+             wndEvalTC p (TApp fn a1 args) (mkApp fn' (tcons a1 args)) )).
+  intros t wih p fn' h1 a1 args h2.
+  destruct h1.
+  - constructor. apply sAppFn; try assumption.
+    eapply WFApp_goodFn. eassumption.
+  - apply wih.
+
+
+induction 1; intros.
+- constructor. apply sAppFn. assumption. inversion H0.
+  + destruct H1. unfold isApp. exists t, a1, args. reflexivity.
+  + assumption.
+- eapply wETCtrn. 
+  + apply IHwndEvalTC1. assumption.
+  + assert (j:= wndEvalTC_WFApp H). apply IHwndEvalTC2. assumption.
+
+
+rewrite mkApp_goodFn; trivial.
+  apply sAppFn; assumption.
+- eapply wERTCtrn. 
+  + apply IHwndEvalRTC1. assumption.
+  + apply IHwndEvalRTC2. assumption.
+Qed.
+***)
+
+(***
+Lemma wndEvalRTC_App_fn:
+  forall p fn fn', wndEvalRTC p fn fn' ->
+    forall a1 args, WFapp (TApp fn a1 args) ->
+    (~ isApp fn' /\ wndEval p (TApp fn a1 args) (TApp fn' a1 args)) \/
+    (isApp fn' /\ wndEval p (TApp fn a1 args) (mkApp fn' (tcons a1 args))). 
+Proof.
+***)
+
+(*** HERE is another version of the problem  ***)
+Lemma wndEvalRTC_App_fn:
+  forall p fn fn', wndEvalRTC p fn fn' -> WFaEnv p ->
+    forall  a1 args, 
+      wndEvalRTC p (mkApp fn (tcons a1 args)) (mkApp fn' (tcons a1 args)).
+induction 1; intros.
+- apply wERTCrfl. 
+- apply wERTCstep. eapply wndEval_mkApp_mkApp. assumption.
+- eapply wERTCtrn. eapply IHwndEvalRTC1; assumption.
+  eapply IHwndEvalRTC2. assumption. 
+Qed.
+
+
+Lemma wndEvalRTC_App_arg:
+  forall p fn arg arg',
+    wndEvalRTC p arg arg' -> ~ isApp fn ->
+    forall args, 
+      wndEvalRTC p (TApp fn arg args) (TApp fn arg' args).
+induction 1; intros h args.
+- constructor.
+- constructor. apply sAppArg; assumption.
+- eapply wERTCtrn;
+  try apply IHwndEvalRTC1; try apply IHwndEvalRTC2; assumption.
+Qed.
+
+Lemma wndEvalTC_App_arg:
+  forall p fn arg arg',
+    wndEvalTC p arg arg' ->
+    forall args, 
+      wndEvalTC p (TApp fn arg args) (TApp fn arg' args).
+induction 1; intros args.
+- constructor. apply sAppArg. assumption.
+- eapply wETCtrn. apply IHwndEvalTC1. apply IHwndEvalTC2.
+Qed.
+
+Lemma wndEvalsRTC_App_args:
+  forall p fn arg args args',
+    wndEvalsRTC p args args' -> ~ isApp fn ->
+      wndEvalRTC p (TApp fn arg args) (TApp fn arg args').
+induction 1; intros h.
+- constructor.
+- constructor. apply sAppArgs; assumption.
+- eapply wERTCtrn. apply IHwndEvalsRTC1. assumption. 
+  apply IHwndEvalsRTC2. assumption. 
+Qed.
+
+Lemma wndEvalsTC_App_args:
+  forall p fn arg args args',
+    wndEvalsTC p args args' -> ~ isApp fn ->
+      wndEvalTC p (TApp fn arg args) (TApp fn arg args').
+induction 1; intros h.
+- constructor. apply sAppArgs; assumption.
+- eapply wETCtrn. apply IHwndEvalsTC1. assumption. 
+  apply IHwndEvalsTC2. assumption. 
+Qed.
+
+Lemma wndEvalRTC_Lam_typ:
+  forall p ty ty',
+    wndEvalRTC p ty ty' ->
+    forall nm bod, 
+      wndEvalRTC p (TLambda nm ty bod) (TLambda nm ty' bod).
+induction 1; intros nm bod.
+- constructor.
+- constructor. apply sLamTy. assumption.
+- eapply wERTCtrn. apply IHwndEvalRTC1. apply IHwndEvalRTC2.
+Qed.
+
+Lemma wndEvalRTC_Prod_typ:
+  forall p ty ty',
+    wndEvalRTC p ty ty' ->
+    forall nm bod, 
+      wndEvalRTC p (TProd nm ty bod) (TProd nm ty' bod).
+induction 1; intros nm bod.
+- constructor.
+- constructor. apply sProdTy. assumption.
+- eapply wERTCtrn. apply IHwndEvalRTC1. apply IHwndEvalRTC2.
+Qed.
+
+Lemma wndEvalRTC_LetIn_dfn:
+  forall p nm dfn dfn',
+    wndEvalRTC p dfn dfn' ->
+    forall ty bod, 
+      wndEvalRTC p (TLetIn nm dfn ty bod) (TLetIn nm dfn' ty bod).
+induction 1; intros ty bod.
+- constructor.
+- constructor. apply sLetInDef. assumption.
+- eapply wERTCtrn. apply IHwndEvalRTC1. apply IHwndEvalRTC2.
+Qed.
+
+Lemma wndEvalTC_LetIn_dfn:
+  forall p nm dfn dfn',
+    wndEvalTC p dfn dfn' ->
+    forall ty bod, 
+      wndEvalTC p (TLetIn nm dfn ty bod) (TLetIn nm dfn' ty bod).
+induction 1; intros ty bod.
+- constructor. apply sLetInDef. assumption.
+- eapply wETCtrn. apply IHwndEvalTC1. apply IHwndEvalTC2.
+Qed.
+
+Lemma wndEvalRTC_Case_mch:
+  forall p mch mch',
+    wndEvalRTC p mch mch' -> 
+    forall np ty brs, 
+      wndEvalRTC p (TCase np ty mch brs) (TCase np ty mch' brs).
+induction 1; intros.
+- constructor.
+- constructor. apply sCaseArg. assumption.
+- eapply wERTCtrn. apply IHwndEvalRTC1. apply IHwndEvalRTC2.
+Qed.
+
+Lemma wndEvalTC_Case_mch:
+  forall p mch mch',
+    wndEvalTC p mch mch' -> 
+    forall np ty brs, 
+      wndEvalTC p (TCase np ty mch brs) (TCase np ty mch' brs).
+induction 1; intros.
+- constructor. apply sCaseArg. assumption.
+- eapply wETCtrn. apply IHwndEvalTC1. apply IHwndEvalTC2.
+Qed.
+
+Lemma wndEvalsRTC_tcons_hd:
+  forall p t t' ts,
+    wndEvalRTC p t t' -> wndEvalsRTC p (tcons t ts) (tcons t' ts).
+induction 1.
+- constructor.
+- constructor. apply saHd. assumption.
+- eapply wEsRTCtrn. apply IHwndEvalRTC1. apply IHwndEvalRTC2.
+Qed.
+
+Lemma wndEvalsTC_tcons_hd:
+  forall p t t' ts,
+    wndEvalTC p t t' -> wndEvalsTC p (tcons t ts) (tcons t' ts).
+induction 1.
+- constructor. apply saHd. assumption.
+- eapply wEsTCtrn. apply IHwndEvalTC1. apply IHwndEvalTC2.
+Qed.
+
+Lemma wndEvalsRTC_tcons_tl:
+  forall p t ts ts',
+    wndEvalsRTC p ts ts' -> wndEvalsRTC p (tcons t ts) (tcons t ts').
+induction 1.
+- constructor.
+- constructor. apply saTl. assumption.
+- eapply wEsRTCtrn. apply IHwndEvalsRTC1. apply IHwndEvalsRTC2.
+Qed.
+
+Lemma wndEvalsTC_tcons_tl:
+  forall p t ts ts',
+    wndEvalsTC p ts ts' -> wndEvalsTC p (tcons t ts) (tcons t ts').
+induction 1.
+- constructor. apply saTl. assumption.
+- eapply wEsTCtrn. apply IHwndEvalsTC1. apply IHwndEvalsTC2.
+Qed.
+
+
+Lemma wndEval_weaken:
+  forall p,
+  (forall t s, wndEval p t s -> forall nm ec, fresh nm p ->
+                   wndEval ((nm,ec)::p) t s) /\
+  (forall ts ss, wndEvals p ts ss -> forall nm ec, fresh nm p ->
+                    wndEvals ((nm,ec)::p) ts ss).
+intros p. apply wndEvalEvals_ind; intros; auto. 
+- apply sConst. apply Lookup_weaken; assumption.
+- eapply sCasen; eassumption.
+Qed.
+
+Lemma wndEval_strengthen:
+  forall (pp:environ),
+  (forall t s, wndEval pp t s -> forall nm ec p, pp = (nm,ec)::p ->
+        ~ PoccTrm nm t -> wndEval p t s) /\
+  (forall ts ss, wndEvals pp ts ss -> forall nm ec p, pp = (nm,ec)::p ->
+        ~ PoccTrms nm ts -> wndEvals p ts ss).
+intros pp. apply wndEvalEvals_ind; intros; auto.
+- apply sConst. 
+  assert (j:= neq_sym (inverse_Pocc_TConstL H0)). inversion_Clear l.
+  + injection H2; intros. contradiction.
+  + injection H4; intros. subst. assumption.
+- eapply sCasen; eassumption.
+- apply sAppFn; trivial. apply (H nm ec). trivial.
+  apply (proj1 (notPocc_mkApp _ _ H1)). 
+- apply sAppArg. apply (H nm ec); trivial. apply (notPocc_TApp H1).
+- apply sAppArgs. apply (H nm ec); trivial. apply (notPocc_TApp H1).
+- apply sProdTy. apply (H nm0 ec); trivial; apply (notPocc_TProd H1).
+- apply sLamTy. apply (H nm0 ec); trivial; apply (notPocc_TLambda H1).
+- apply sLetInTy. apply (H nm0 ec); trivial; apply (notPocc_TLetIn H1).
+- apply sLetInDef. apply (H nm0 ec); trivial; apply (notPocc_TLetIn H1).
+- apply sCaseTy. apply (H nm ec); trivial; apply (notPocc_TCase H1).
+- apply sCaseArg. apply (H nm ec); trivial; apply (notPocc_TCase H1).
+- apply sCaseBrs. apply (H nm ec); trivial; apply (notPocc_TCase H1).
+- apply saHd. apply (H nm ec). trivial. apply (notPoccTrms H1).
+- apply saTl. apply (H nm ec). trivial. apply (notPoccTrms H1).
+Qed.
+
+***)
