Randy_8.5beta2/RandyWorking/L1_MalechaQuoted/wcbvEval.v
@@ -1,0 +1,1419 @@
+Add LoadPath "../common" as Common.
+Add LoadPath "." as L1.
+Require Import Lists.List.
+Require Import Strings.String.
+Require Import Arith.Compare_dec.
+Require Import Program.Basics.
+Require Import Omega.
+Require Import Logic.JMeq.
+Require Import L1.term.
+Require Import L1.program.
+Require Import L1.wndEval.
+Require Import L1.awndEval.
+
+Local Open Scope string_scope.
+Local Open Scope bool.
+Local Open Scope list.
+Set Implicit Arguments.
+
+(** Relational version of weak cbv evaluation  **)
+Inductive WcbvEval (p:environ) : Term -> Term -> Prop :=
+| wLam: forall nm ty ty' bod,
+          WcbvEval p ty ty' ->
+          WcbvEval p (TLambda nm ty bod) (TLambda nm ty' bod)
+| wProd: forall nm ty ty' bod,
+          WcbvEval p ty ty' ->
+          WcbvEval p (TProd nm ty bod) (TProd nm ty' bod)
+| wCast: forall t s ck ty,
+          WcbvEval p t s -> WcbvEval p (TCast t ck ty) s
+| wConstruct: forall i r, WcbvEval p (TConstruct i r) (TConstruct i r)
+| wInd: forall i, WcbvEval p (TInd i) (TInd i) 
+| wSort: forall srt, WcbvEval p (TSort srt) (TSort srt)
+| wFix: forall dts m, WcbvEval p (TFix dts m) (TFix dts m)
+| wConst: forall nm (t s:Term),
+            LookupDfn nm p t -> WcbvEval p t s -> WcbvEval p (TConst nm) s
+| wAppLam: forall (fn ty bod a1 a1' s:Term) (args:Terms) (nm:name),
+               WcbvEval p fn (TLambda nm ty bod) ->
+               WcbvEval p a1 a1' ->
+               WcbvEval p (whBetaStep bod a1' args) s ->
+               WcbvEval p (TApp fn a1 args) s
+| wLetIn: forall (nm:name) (dfn ty bod dfn' s:Term),
+            WcbvEval p dfn dfn' ->
+            WcbvEval p (instantiate dfn' 0 bod) s ->
+            WcbvEval p (TLetIn nm dfn ty bod) s
+| wAppFix: forall dts m (fn arg fs s:Term) (args:Terms),
+               WcbvEval p fn (TFix dts m) ->
+               whFixStep dts m (tcons arg args) = Some fs ->
+               WcbvEval p fs s ->
+               WcbvEval p (TApp fn arg args) s
+| wAppCnstr: forall fn i n arg arg1 args args1,
+               WcbvEval p fn (TConstruct i n) ->
+               WcbvEval p arg arg1 ->
+               WcbvEvals p args args1 ->
+               WcbvEval p (TApp fn arg args)
+                        (TApp (TConstruct i n) arg1 args1)
+| wAppInd: forall fn i arg arg1 args args1,
+               WcbvEval p fn (TInd i) ->
+               WcbvEval p arg arg1 ->
+               WcbvEvals p args args1 ->
+               WcbvEval p (TApp fn arg args)
+                        (TApp (TInd i) arg1 args1)
+| wCase0: forall mch i n ty brs cs s,
+           WcbvEval p mch (TConstruct i n) ->
+           whCaseStep n tnil brs = Some cs ->
+           WcbvEval p cs s ->
+           WcbvEval p (TCase 0 ty mch brs) s
+| wCasen: forall mch i n ty arg args np brs cs s ts,
+           WcbvEval p mch (TApp (TConstruct i n) arg args) ->
+           tskipn np (tcons arg args) = Some ts ->
+           whCaseStep n ts brs = Some cs ->
+           WcbvEval p cs s ->
+           WcbvEval p (TCase np ty mch brs) s
+with WcbvEvals (p:environ) : Terms -> Terms -> Prop :=
+| wNil: WcbvEvals p tnil tnil
+| wCons: forall t t' ts ts',
+           WcbvEval p t t' -> WcbvEvals p ts ts' -> 
+           WcbvEvals p (tcons t ts) (tcons t' ts').
+Hint Constructors WcbvEval WcbvEvals.
+Scheme WcbvEval1_ind := Induction for WcbvEval Sort Prop
+  with WcbvEvals1_ind := Induction for WcbvEvals Sort Prop.
+Combined Scheme WcbvEvalEvals_ind from WcbvEval1_ind, WcbvEvals1_ind.
+
+(** evaluate omega = (\x.xx)(\x.xx): nontermination **)
+Definition xx := (TLambda nAnon prop (TApp (TRel 0) (TRel 0) tnil)).
+Definition xxxx := (TApp xx xx tnil).
+Goal WcbvEval nil xxxx xxxx.
+unfold xxxx, xx.
+eapply wAppLam. eapply wLam. eapply wSort. eapply wLam. eapply wSort.
+unfold whBetaStep, instantiate.
+rewrite (proj2 (nat_compare_eq_iff 0 0) eq_refl).
+rewrite mkApp_idempotent. rewrite mkApp_idempotent. simpl.
+change (WcbvEval nil xxxx xxxx).
+Abort.
+
+
+Lemma WcbvEval_mkApp_nil:
+  forall t, WFapp t -> forall p s, WcbvEval p t s ->
+                 WcbvEval p (mkApp t tnil) s.
+Proof.
+  intros p. induction 1; simpl; intros; try assumption.
+  - rewrite tappend_tnil. assumption.
+Qed.
+
+
+(** wcbvEval preserves WFapp **)
+Lemma wcbvEval_pres_WFapp:
+  forall p, WFaEnv p -> 
+  (forall t s, WcbvEval p t s -> WFapp t -> WFapp s) /\
+  (forall ts ss, WcbvEvals p ts ss -> WFapps ts -> WFapps ss).
+Proof.
+  intros p hp. apply WcbvEvalEvals_ind; intros; try assumption.
+  - inversion_Clear H0. intuition.
+  - inversion_Clear H0. intuition.
+  - inversion_Clear H0. apply H. assumption.
+  - inversion_Clear H0. apply H.
+    assert (j:= Lookup_pres_WFapp hp l). inversion j. assumption.
+  - inversion_Clear H2. apply H1.
+    apply (whBetaStep_pres_WFapp); try assumption.
+    + assert (j:= H H7). inversion_Clear j. assumption.
+    + apply H0. assumption. 
+  - inversion_Clear H1. apply H0. apply instantiate_pres_WFapp. assumption.
+    + apply H. assumption.
+  - inversion_Clear H1. apply H0. unfold whFixStep in e.
+    assert (k:= H H6). inversion_Clear k.
+    assert (j:= dnthBody_pres_WFapp H2 m). destruct (dnthBody m dts).
+    + injection e. intros. rewrite <- H1. apply mkApp_pres_WFapp.
+      * constructor; assumption.
+      * { apply fold_left_pres_WFapp. intros.
+          - apply instantiate_pres_WFapp. assumption.
+            + constructor. assumption. 
+          - apply j. reflexivity. }
+    + discriminate.
+  - inversion_Clear H2. apply wfaApp; try intuition. 
+    + destruct H2 as [x0 [x1 [x2 j]]]. discriminate.
+  - inversion_Clear H2. apply wfaApp; try intuition. 
+    + destruct H2 as [x0 [x1 [x2 j]]]. discriminate.
+  - apply H0. inversion_Clear H1.
+    refine (whCaseStep_pres_WFapp _ _ _ e); auto.
+  - apply H0. inversion_Clear H1.
+    refine (whCaseStep_pres_WFapp _ _ _ e0); auto.
+    assert (j:= H H5). inversion_Clear j.
+    refine (tskipn_pres_WFapp _ _ e). intuition.
+  - inversion_Clear H1. intuition. 
+Qed.
+
+
+Lemma WcbvEval_weaken:
+  forall p,
+  (forall t s, WcbvEval p t s -> forall nm ec, fresh nm p ->
+                   WcbvEval ((nm,ec)::p) t s) /\
+  (forall ts ss, WcbvEvals p ts ss -> forall nm ec, fresh nm p ->
+                    WcbvEvals ((nm,ec)::p) ts ss).
+intros p. apply WcbvEvalEvals_ind; intros; auto.
+- eapply wConst. 
+  + apply Lookup_weaken; eassumption.
+  + apply H. assumption.
+- eapply wAppLam.
+  + apply H. assumption.
+  + apply H0. assumption.
+  + apply H1. assumption.
+- eapply wLetIn.
+  + apply H. assumption.
+  + apply H0. assumption.
+- eapply wAppFix.
+  + apply H. assumption.
+  + apply e.
+  + apply H0. assumption.
+- eapply wCase0.
+  + apply H. assumption.
+  + apply e.
+  + apply H0. assumption.
+- eapply wCasen.
+  + apply H. assumption.
+  + apply e.
+  + apply e0.
+  + apply H0. assumption.
+Qed.
+
+(****  Could probably finish this, bus see WcbvEval_wndEvalRTC below ***
+(** WcbvEval is in the transitive closure of wndEval **)
+Lemma WcbvEval_wndEvalTC:
+  forall (p:environ), WFaEnv p ->
+    (forall t s, WcbvEval p t s -> t <> s ->
+        WFapp t -> wndEvalTC p t s) /\
+    (forall ts ss, WcbvEvals p ts ss -> ts <> ss ->
+        WFapps ts -> wndEvalsTC p ts ss).
+Proof.
+  intros p hp. apply WcbvEvalEvals_ind; intros; try (nreflexivity H).
+  - destruct (Term_dec t s).
+    + apply wETCstep. subst. apply sCast.
+    + inversion_Clear H1. eapply wETCtrn.
+      * apply wETCstep. apply sCast.
+      * eapply H; eassumption.
+  - destruct (Term_dec t s).
+    + apply wETCstep. subst. apply (sConst l). 
+    + eapply wETCtrn.
+      * apply wETCstep. constructor. eassumption.
+      * eapply H. eassumption.
+        assert (j:= Lookup_pres_WFapp hp l). inversion j. assumption.
+  - destruct (Term_dec fn (TLambda nm ty bod)), (Term_dec a1 a1'),
+    (Term_dec (whBetaStep bod a1' args) s). subst.
+    + apply wETCstep. constructor.
+    + eapply wETCtrn.
+      * apply wETCstep. constructor.
+      * eapply H1. eassumption.
+        inversion_Clear H3. inversion_Clear H9.
+        apply whBetaStep_pres_WFapp; assumption.
+    + eapply wETCtrn.
+      * inversion_Clear H3. 
+        apply wndEvalTC_App_arg. apply H0; assumption. 
+      * apply wETCstep. apply sBeta.
+    + eapply wETCtrn. 
+      * apply wndEvalTC_App_arg.
+        inversion_Clear H3. inversion_Clear H10.
+        eapply H0; eassumption.
+      * eapply wETCtrn. constructor. constructor. eapply H1. assumption.
+        inversion_Clear H3. inversion_Clear H10.
+        apply whBetaStep_pres_WFapp; try eassumption.
+        eapply (proj1 (wcbvEval_pres_WFapp hp)); eassumption.
+    + eapply wETCtrn. apply wndEval_App_fn.
+
+
+
+ (** HERE **) apply wndEvalTC_App_fn. apply H; assumption.
+    constructor. constructor.
+  + eapply wETCtrn. apply wndEvalTC_App_fn. apply H; assumption.
+    eapply wETCtrn. constructor. constructor. apply H1; assumption.
+  + eapply wETCtrn. apply wndEvalTC_App_fn. apply H; assumption.
+    eapply wETCtrn. apply wndEvalTC_App_arg. apply H0. assumption.
+    constructor. constructor.
+  + eapply wETCtrn. apply wndEvalTC_App_fn. apply H; assumption.
+    eapply wETCtrn. apply wndEvalTC_App_arg. apply H0. assumption.
+    eapply wETCtrn. constructor. constructor.
+    apply H1. assumption.
+- destruct (Term_dec dfn dfn');
+  destruct (Term_dec (instantiate dfn' 0 bod) s); subst.
+  + apply wETCstep. constructor.
+  + eapply wETCtrn. apply wETCstep. constructor. apply H0. assumption.
+  + eapply wETCtrn. apply wndEvalTC_LetIn_dfn. apply H. assumption.
+    constructor. constructor.
+  + eapply wETCtrn. apply wndEvalTC_LetIn_dfn. apply H. assumption.
+    eapply wETCtrn. constructor. constructor.
+    apply H0. assumption.
+- destruct (Term_dec fn (TFix dts m)); destruct (Term_dec fs s); subst.
+  + apply wETCstep. constructor. assumption.
+  + eapply wETCtrn. apply wETCstep. constructor. eassumption.
+    apply H0. assumption.
+  + eapply wETCtrn. apply wndEvalTC_App_fn. apply H. assumption.
+    constructor. constructor. assumption.
+  + eapply wETCtrn. apply wndEvalTC_App_fn. apply H. assumption.
+    eapply wETCtrn. constructor. constructor. eassumption.
+    apply H0. assumption.
+- destruct (Term_dec fn (TConstruct i r)); destruct (Term_dec arg arg');
+  destruct (Terms_dec args args'); subst.
+  + elim H2. reflexivity.
+  + apply wndEvalsTC_App_args. apply H1. assumption.
+  + apply wndEvalTC_App_arg. apply H0. assumption.
+  + eapply wETCtrn. apply wndEvalTC_App_arg. apply H0. assumption.
+    apply wndEvalsTC_App_args. apply H1. assumption.
+  + apply wndEvalTC_App_fn. apply H. assumption.
+  + eapply wETCtrn. apply wndEvalTC_App_fn. apply H. assumption.
+    apply wndEvalsTC_App_args. apply H1. assumption.
+  + eapply wETCtrn. apply wndEvalTC_App_fn. apply H. assumption.
+    apply wndEvalTC_App_arg. apply H0. assumption.
+  + eapply wETCtrn. apply wndEvalTC_App_fn. apply H. assumption.
+    eapply wETCtrn. apply wndEvalTC_App_arg. apply H0. assumption.
+    apply wndEvalsTC_App_args. apply H1. assumption.
+
+
+
+-
+
+- apply H. assumption.
+ eapply wERTCtrn. apply wERTCstep. apply sConst. eassumption.
+  assumption.
+- eapply (@wERTCtrn _ _ (TApp (TLambda nm ty bod) a1 args)).
+  + apply wndEvalRTC_App_fn. assumption.
+  + eapply (@wERTCtrn _ _ (TApp (TLambda nm ty bod) a1' args)).
+    * apply wndEvalRTC_App_arg. assumption.
+    * apply (@wERTCtrn _ _ (whBetaStep bod a1' args)).
+      apply wERTCstep. apply sBeta. assumption.
+- eapply (@wERTCtrn _ _ (TLetIn nm dfn' ty bod)).
+  + apply wndEvalRTC_LetIn_dfn. assumption.
+  + eapply wERTCtrn. apply wERTCstep. apply sLetIn. assumption.
+- eapply (@wERTCtrn _ _ (TApp (TFix dts m) arg args)).
+  + apply wndEvalRTC_App_fn. assumption.
+  + eapply (@wERTCtrn _ _ fs).
+    * apply wERTCstep. apply sFix. assumption.
+    * assumption.
+- eapply (@wERTCtrn _ _ (TApp (TConstruct i r) arg args)).
+  + apply wndEvalRTC_App_fn. assumption.
+  + eapply (@wERTCtrn _ _ (TApp (TConstruct i r) arg' args)).
+    * apply wndEvalRTC_App_arg. assumption.
+    * eapply (@wERTCtrn _ _ (TApp (TConstruct i r) arg' args')).
+      apply wndEvalsRTC_App_args. assumption.
+      constructor.
+- eapply (@wERTCtrn _ _ (TCase 0 ty (TConstruct i n) brs)).
+  + apply wndEvalRTC_Case_mch. assumption.
+  + eapply (@wERTCtrn _ _ cs).
+    * apply wERTCstep. apply sCase0. assumption.
+    * assumption.
+- eapply (@wERTCtrn _ _ (TCase np ty (TApp (TConstruct i n) arg args) brs)).
+  + apply wndEvalRTC_Case_mch. assumption.
+  + eapply (@wERTCtrn _ _ cs).
+    * apply wERTCstep. eapply sCasen; eassumption.
+    * assumption.
+- eapply (@wEsRTCtrn _ _ (tcons t' ts)).
+  + apply wndEvalsRTC_tcons_hd. assumption.
+  +  eapply (@wEsRTCtrn _ _ (tcons t' ts')).
+     * apply wndEvalsRTC_tcons_tl. assumption.
+     * constructor.
+Qed.
+*******)
+
+Lemma WcbvEval_wndEvalRTC:
+  forall (p:environ), WFaEnv p ->
+    (forall t s, WcbvEval p t s -> WFapp t -> wndEvalRTC p t s) /\
+    (forall ts ss, WcbvEvals p ts ss -> WFapps ts -> wndEvalsRTC p ts ss).
+intros p hp. apply WcbvEvalEvals_ind; intros; try (solve [constructor]).
+- inversion_Clear H0. 
+  eapply wERTCtrn. 
+  + apply wndEvalRTC_Lam_typ. eapply H. assumption.
+  + constructor. 
+- inversion_Clear H0. 
+  eapply wERTCtrn. 
+  + apply wndEvalRTC_Prod_typ. eapply H. assumption.
+  + constructor. 
+- eapply wERTCtrn. apply wERTCstep. apply sCast. apply H. 
+  inversion_Clear H0. assumption.
+- eapply wERTCtrn. 
+  + apply wERTCstep. apply sConst. eassumption.
+  + apply H. assert (j:= Lookup_pres_WFapp hp l). inversion j. assumption.
+- eapply (@wERTCtrn _ _ (TApp (TLambda nm ty bod) a1 args));
+  inversion_Clear H2. 
+  + rewrite <- mkApp_goodFn; try assumption.
+    rewrite <- mkApp_goodFn; try not_isApp.
+    apply wndEvalRTC_App_fn. apply H. assumption. assumption.
+  + eapply (@wERTCtrn _ _ (TApp (TLambda nm ty bod) a1' args)).
+    * apply wndEvalRTC_App_arg. apply H0. assumption. not_isApp.
+    * { apply (@wERTCtrn _ _ (whBetaStep bod a1' args)).
+        - apply wERTCstep. apply sBeta. 
+        - apply H1. apply whBetaStep_pres_WFapp; try eassumption.
+          + assert (j:= proj1 (wcbvEval_pres_WFapp hp) _ _ w H7).
+            inversion_Clear j. assumption.
+          + eapply wndEvalRTC_pres_WFapp; try eassumption.
+            * apply H0. assumption. }
+- inversion_Clear H1. eapply (@wERTCtrn _ _ (TLetIn nm dfn' ty bod)).
+  + apply wndEvalRTC_LetIn_dfn. intuition.
+  + eapply wERTCtrn. apply wERTCstep. apply sLetIn. apply H0.
+    apply instantiate_pres_WFapp; try assumption.
+    * eapply (proj1 (wcbvEval_pres_WFapp hp)); try eassumption.
+- inversion_Clear H1.
+  refine (@wERTCtrn _ _ (TApp (TFix dts m) arg args) _ _ _).
+  + rewrite <- mkApp_goodFn; try assumption.
+    rewrite <- mkApp_goodFn; try not_isApp.
+    apply wndEvalRTC_App_fn. apply H. assumption. assumption.
+  + refine (@wERTCtrn _ _ fs _ _ _).
+    * apply wERTCstep. apply sFix. assumption.
+    * { apply H0. refine (whFixStep_pres_WFapp _ _ _ e); try eassumption.
+        - assert (j:= wndEvalRTC_pres_WFapp (H H6) hp H6).
+          inversion_Clear j. assumption.
+        - constructor; assumption. }
+- inversion_Clear H2.
+  eapply (@wERTCtrn _ _ (TApp (TConstruct i n) arg args)).
+  + rewrite <- mkApp_goodFn; try assumption.
+    rewrite <- mkApp_goodFn; try not_isApp.
+    apply wndEvalRTC_App_fn. apply H. assumption. assumption.
+  + eapply (@wERTCtrn _ _ (TApp (TConstruct i n) arg1 args)).
+    * { apply wndEvalRTC_App_arg; try not_isApp.
+        - apply H0. assumption. }
+    * { eapply (@wERTCtrn _ _ (TApp (TConstruct i n) arg1 args1)).
+        - apply wndEvalsRTC_App_args; try not_isApp.
+          + apply H1. assumption. 
+        - apply wERTCrfl. }
+- inversion_Clear H2.
+  eapply (@wERTCtrn _ _ (TApp (TInd i) arg args)).
+  + rewrite <- mkApp_goodFn; try assumption.
+    rewrite <- mkApp_goodFn; try not_isApp.
+    apply wndEvalRTC_App_fn. apply H. assumption. assumption.
+  + eapply (@wERTCtrn _ _ (TApp (TInd i) arg1 args)).
+    * { apply wndEvalRTC_App_arg; try not_isApp.
+        - apply H0. assumption. }
+    * { eapply (@wERTCtrn _ _ (TApp (TInd i) arg1 args1)).
+        - apply wndEvalsRTC_App_args; try not_isApp.
+          + apply H1. assumption. 
+        - apply wERTCrfl. }
+- inversion_Clear H1. eapply wERTCtrn. 
+  + eapply wndEvalRTC_Case_mch. apply H. assumption.
+  + eapply (@wERTCtrn _ _ cs). 
+    * apply wERTCstep. apply sCase0. assumption.
+    * { apply H0. eapply whCaseStep_pres_WFapp.
+        - eapply H7.
+        - eapply wfanil.
+        - eassumption. }
+- inversion_Clear H1. eapply wERTCtrn. 
+  + eapply wndEvalRTC_Case_mch. apply H. assumption.
+  + eapply (@wERTCtrn _ _ cs). 
+    * apply wERTCstep. eapply sCasen; eassumption.
+    * { apply H0. eapply whCaseStep_pres_WFapp.
+        - eapply H7.
+        - assert (j: WFapps (tcons arg args)).
+          { assert (k:= proj1 (wcbvEval_pres_WFapp hp) _ _ w H5).
+            inversion_clear k. constructor; assumption. }
+          eapply tskipn_pres_WFapp. apply j. eassumption. 
+        - eassumption. }
+- inversion_Clear H1. eapply (@wEsRTCtrn _ _ (tcons t' ts)).
+  + apply wndEvalsRTC_tcons_hd. apply H. assumption.
+  + eapply (@wEsRTCtrn _ _ (tcons t' ts')).
+     * apply wndEvalsRTC_tcons_tl. apply H0. assumption.
+     * apply wEsRTCrfl.
+Qed.
+
+
+(************  in progress  ****
+Lemma WcbvEval_strengthen:
+  forall pp,
+  (forall t s, WcbvEval pp t s -> forall nm u p, pp = (nm,ecConstr u)::p ->
+        ~ PoccTrm nm t -> WcbvEval p t s) /\
+  (forall ts ss, WcbvEvals pp ts ss -> forall nm u p, pp = (nm,ecConstr u)::p ->
+        ~ PoccTrms nm ts -> WcbvEvals p ts ss).
+intros pp. apply WcbvEvalEvals_ind; intros; auto.
+- eapply (@wConst p nm t s pp). eapply (@Lookup_strengthen _ pp); try eassumption.
+  + apply (neq_sym (inverse_Pocc_TConstL H1)).
+  + eapply H. eassumption.
+    admit.
+- Check (deMorgan_impl (@PoAppL _ _ _ _) H3).
+  assert (hfn:= deMorgan_impl (@PoAppL _ _ _ _) H3).
+  assert (harg:= deMorgan_impl (@PoAppA _ _ _ _) H3).
+  assert (hargs:= deMorgan_impl (@PoAppR _ _ _ _) H3).
+  eapply wAppLam. 
+  + eapply H; eassumption.
+  + eapply H0; eassumption.
+  + eapply H1. eassumption. intros j.
+
+
+
+rewrite H0 in l. assert (j:= proj2 (lookupDfn_LookupDfn _ _ _) l).
+  simpl in j.
+  rewrite (string_eq_bool_neq (neq_sym (inverse_Pocc_TConstL H1))) in j. 
+Check (@wConst p _ t).
+  eapply (@wConst p _ t).
+assert (h:= inverse_Pocc_TConstL H1).
+
+rewrite H0 in l. simpl in l. eapply (wConst pp). 
+
+rewrite H0 in H. simpl in H.
+  rewrite (string_eq_bool_neq (neq_sym (inverse_Pocc_TConstL H0))) in e. 
+  trivial.
+- apply (H nm u); trivial. apply (notPocc_TApp H1).
+- apply (H nm u); trivial. apply (notPocc_TApp H1).
+- apply (H nm u); trivial. apply (notPocc_TApp H1).
+- apply (H nm0 u); trivial; apply (notPocc_TProd H1).
+- apply (H nm0 u); trivial; apply (notPocc_TLambda H1).
+- apply (H nm0 u); trivial; apply (notPocc_TLetIn H1).
+- apply (H nm0 u); trivial; apply (notPocc_TLetIn H1).
+- apply (H nm u); trivial; apply (notPocc_TCast H1).
+- apply (H nm u); trivial; apply (notPocc_TCast H1).
+- apply (H nm u); trivial; apply (notPocc_TCase H1).
+- apply (H nm u); trivial; apply (notPocc_TCase H1).
+- apply (H nm u); trivial; apply (notPocc_TCase H1).
+- apply (H nm u). trivial. apply (notPoccTrms H1).
+- apply (H nm u). trivial. apply (notPoccTrms H1).
+Qed.
+***************)
+
+(** now an executable weak-call-by-value evaluation **)
+(** use a timer to make this terminate **)
+(****  Working HERE  ****
+Definition wcbvEv:
+  forall (p:environ) (tmr:nat),
+    (forall (t:Term), exception Term) *
+    (forall (ts:Terms), exception Terms) *
+    (forall (ds:Defs), True).
+Proof.
+  intros p t. induction t; intros.
+  Case "tmr = 0". split; split; intros; apply (Exc "out of time").
+  Case "tmr = S n". apply TrmTrmsDefs_Typeind; intros.
+  - SCase "TRel". apply (Exc "TRel; free index").
+  - SCase "TSort". apply (Ret (TSort s)).
+  - SCase "TCast". apply (fst (fst IHt) t0).
+  - SCase "TProd". apply (Ret (TProd n t0 t1)).
+  - SCase "TLambda". apply (Ret (TLambda n t0 t1)).
+  - SCase "TLetIn". destruct H.
+    + apply (Exc s).
+    + destruct (fst (fst IHt) (instantiate t0 0 t2)).
+      * apply (Exc s).
+      * apply (Ret t4).
+  - SCase "TApp". destruct H.
+    + SSCase "fn doesn't eval". apply (Exc s).
+    + SSCase "fn evals to ..". destruct t3.
+      * SSSCase "TRel". apply (Exc "never result of eval").
+      * SSSCase "TSort". apply (Exc "doesn't have functional type").
+      * SSSCase "TCast". apply (Exc "never result of eval").
+      * SSSCase "TProd". apply (Exc "doesn't have functional type").
+      * SSSCase "TLambda". destruct H0.
+        SSSSCase "arg doesn't eval". apply (Exc s).
+        SSSSCase "arg evals". apply (fst (fst IHt) (whBetaStep t3_2 t3 t2)).
+      * SSSCase "TLetIn". apply (Exc "never result of eval").
+      * SSSCase "TApp: must mkApp". 
+        apply (fst (fst IHt) (mkApp t3_1 (tcons t3_2 t3))).
+      * SSSCase "TConst". apply (Exc "never result of eval").
+      * SSSCase "TInd".
+  -
+apply (Exc "").
+      * SSSCase "TLetIn". apply (Exc "").
+      * SSSCase "TApp". apply (Exc "").
+      * SSSCase "TConst". apply (Exc "").
+      * SSSCase "TInd". apply (Exc "").
+      * SSSCase "TConstruct". apply (Exc "").
+      * SSSCase "TCase". apply (Exc "").
+      * SSSCase "TFix". apply (Exc "").
+  - SCase "TConst". destruct (lookupDfn s p).
+    + SSCase "lookup succeeds". apply (IHtmr p
+    + SSCase "lookup fails". apply (Exc "").
+**************************)
+
+Function wcbvEval
+         (tmr:nat) (p:environ) (t:Term) {struct tmr}: exception Term :=
+  (match tmr with 
+     | 0 => raise "out of time"
+     | S n =>
+       (match t with      (** look for a redex **)
+          | TConst nm => match (lookupDfn nm p) with
+                           | Some t => wcbvEval n p t
+                           | None => raise "environment miss"
+                         end
+          | TCast t _ _ =>  wcbvEval n p t
+          | TApp fn a1 args =>
+            (match wcbvEval n p fn with
+               | Exc str => Exc str
+               | Ret efn =>
+                 (match efn with
+                    | TLambda _ _ bod =>
+                      match wcbvEval n p a1 with
+                        | Exc str => Exc str
+                        | Ret wharg => wcbvEval n p (whBetaStep bod wharg args)
+                      end
+                    | TFix dts m =>
+                      match whFixStep dts m (tcons a1 args) with
+                        | None => raise "fixpoint step fail"
+                        | Some fs => wcbvEval n p fs
+                      end
+                    | TConstruct i m =>
+                      match wcbvEval n p a1, wcbvEvals n p args with
+                        | Ret ea1, Ret eargs =>
+                              Ret (TApp (TConstruct i m) ea1 eargs)
+                        | _, _ => raise "arg of constructor fails to compute"
+                      end
+                    | TInd i => 
+                     match wcbvEval n p a1, wcbvEvals n p args with
+                        | Ret ea1, Ret eargs => Ret (TApp (TInd i) ea1 eargs)
+                        | _, _ => raise "arg of Ind fails to compute"
+                      end
+                     | _ => raise "wcbvEval: application"
+                  end)
+             end)
+          | TCase np _ mch brs =>
+            (match wcbvEval n p mch with
+               | Exc str => Exc str
+               | Ret emch =>
+                 (match emch, np with 
+                    | TConstruct _ r, 0 => 
+                      match whCaseStep r tnil brs with
+                        | None => raise "case step fails"
+                        | Some cs => wcbvEval n p cs
+                      end
+                    | TApp (TConstruct _ r) arg args, _ =>
+                      match tskipn np (tcons arg args) with
+                        | None => raise "not enough args for constructor"
+                        | Some ts => match whCaseStep r ts brs with
+                                       | None => raise "case step fails"
+                                       | Some cs => wcbvEval n p cs
+                                     end
+                      end
+                    | _, _ => raise "case match arg not canonical"
+                  end)
+             end)
+          | TLetIn nm df ty bod =>
+            match wcbvEval n p df with
+              | Exc str => Exc str
+              | Ret df' => wcbvEval n p (instantiate df' 0 bod)
+            end
+          | TLambda nn ty t => 
+            match wcbvEval n p ty with
+              | Exc str => Exc str
+              | Ret ty' => ret (TLambda nn ty' t)
+            end
+          | TProd nn ty t =>
+            match wcbvEval n p ty with
+              | Exc str => Exc str
+              | Ret ty' => ret (TProd nn ty' t)
+            end
+          | TFix mfp br => ret (TFix mfp br)
+          (** already in whnf ***)
+          | TConstruct i cn => ret (TConstruct i cn)
+          | TInd i => ret (TInd i)
+          | TSort srt => ret (TSort srt)
+          (** should never appear **)
+          | TRel _ => raise "wcbvEval: unbound Rel"
+        end)
+   end)
+with wcbvEvals (tmr:nat) (p:environ) (ts:Terms) {struct tmr}
+     : exception Terms :=
+       (match tmr with 
+          | 0 => raise "out of time"
+          | S n => match ts with             (** look for a redex **)
+                     | tnil => ret tnil
+                     | tcons s ss =>
+                       match wcbvEval n p s, wcbvEvals n p ss with
+                         | Ret es, Ret ess => ret (tcons es ess)
+                         | _, _ => raise "wcbvEvals fails"
+                       end
+                   end
+        end).
+(**
+Functional Scheme wcbvEval_ind := Induction for wcbvEval Sort Prop
+with wcbvEvals_ind := Induction for wcbvEvals Sort Prop.
+Combined Scheme wcbvEvalEvals_ind from wcbvEval_ind, wcbvEvals_ind.
+**)
+
+(** wcbvEval and WcbvEval are the same relation **)
+(***
+Lemma wcbvEval_WcbvEval:
+  forall p,
+  (forall t n s, wcbvEval n p t = Ret s -> WcbvEval p t s) /\
+  (forall ts n ss, wcbvEvals n p ts = Ret ss -> WcbvEvals p ts ss) /\
+  (forall (ds:Defs) (n:nat), True).
+intros p.
+- eapply(TrmTrmsDefs_ind
+      (fun t => forall n s, wcbvEval n p t = Ret s -> WcbvEval p t s)
+      (fun ts => forall n ss, wcbvEvals n p ts = Ret ss ->
+                              WcbvEvals p ts ss)
+      (fun (ds:Defs) => forall (n:nat), True)); intros; intuition;
+  try (solve [induction n; simpl in *; discriminate]).
+  + induction n0; simpl in *; try discriminate.
+  + induction n; simpl in *; try discriminate.
+    * myInjection H. constructor.
+  + induction n; simpl in *; try discriminate.
+    * constructor. eapply H.  eassumption. 
+  + induction n0; simpl in *; try discriminate.
+    * { case_eq (wcbvEval n0 p t); intros; rewrite H2 in H1. 
+        - discriminate.
+        - myInjection H1. constructor. eapply H. eassumption. }
+  + induction n0; simpl in *; try discriminate.
+    * { case_eq (wcbvEval n0 p t); intros; rewrite H2 in H1. 
+        - discriminate.
+        - myInjection H1. constructor. eapply H. eassumption. }
+  + induction n0; simpl in *; try discriminate.
+    * { case_eq (wcbvEval n0 p t); intros; rewrite H3 in H2.
+        - discriminate.
+        - eapply wLetIn. 
+          + eapply H. eassumption. 
+          + eassumption.
+          apply IHn0. rewrite <- H2. 
+
+assert (j2:= H _ _ Happly IHn. rewrite <- H1.
+  +
+***)
+
+(***
+Lemma wcbvEval_mono:
+  forall p n t s, wcbvEval n p t = Ret s -> wcbvEval (S n) p t = Ret s.
+Proof.
+  induction t; intros.
+  - simpl in H
+
+
+Lemma wcbvEval_WcbvEval:
+  forall p n,
+  (forall t s, wcbvEval n p t = Ret s -> WcbvEval p t s) /\
+  (forall ts ss, wcbvEvals n p ts = Ret ss -> WcbvEvals p ts ss) /\
+  (forall (ds:Defs), True).
+intros p. induction n.
+- split; try split; simpl; intros; auto; try discriminate.
+- eapply(TrmTrmsDefs_ind
+      (fun t => forall s, wcbvEval (S n) p t = Ret s -> WcbvEval p t s)
+      (fun ts => forall ss, wcbvEvals (S n) p ts = Ret ss -> WcbvEvals p ts ss)
+      (fun (ds:Defs) => True));
+  intuition; simpl; intros; try discriminate;
+  try (solve [myInjection H0; constructor]).
+  + simpl in H4. case_eq (wcbvEval n p t); intros tt h; rewrite h in H4.
+    * discriminate.
+    * myInjection H4. constructor. apply H. assumption.
+  + simpl in H4. case_eq (wcbvEval n p t); intros tt h; rewrite h in H4.
+    * discriminate.
+    * myInjection H4. constructor. apply H. assumption.
+  + simpl in H5. case_eq (wcbvEval n p t); intros tt h; rewrite h in H5.
+    * discriminate.
+    * { case_eq (wcbvEval n p (instantiate tt 0 t1)); intros; rewrite H6 in H5. 
+        - discriminate.
+        - myInjection H5. eapply wLetIn. 
+          + apply H. eassumption.
+          + apply H. assumption. }
+  + simpl in H5. case_eq (wcbvEval n p t); intros tt h; rewrite h in H5.
+    * discriminate.
+    * { case_eq tt; intros; subst; try discriminate.
+        - case_eq (wcbvEval n p t0); intros ttt hh; rewrite hh in H5.
+          + discriminate.
+          + eapply wAppLam. apply H0.
+
+rewrite <- H5. unfold wcbvEval.
+
+  + eapply wAppLam. constructor. apply H. 
+
+
+unfold whBetaStep. instantiate. 
+
+(** wcbvEval and WcbvEval are the same relation **)
+Lemma wcbvEval_WcbvEval:
+  forall n p,
+  (forall t s, wcbvEval n p t = Ret s -> WcbvEval p t s) /\
+  (forall ts ss, wcbvEvals n p ts = Ret ss -> WcbvEvals p ts ss).
+intros n p.
+apply (wcbvEvalEvals_ind 
+  (fun n p t o => forall s, o = Ret s -> WcbvEval p t s)
+  (fun n p ts os => forall ss, os = Ret ss -> WcbvEvals p ts ss));
+  intros; try discriminate;
+  try (solve [injection H; intros h; subst; constructor]).
+- apply wCast. intuition.
+- injection H0. intros. subst. eapply wProd. apply H. assumption.
+- injection H0. intros. subst. eapply wLam. apply H. assumption.
+- eapply wLetIn.
+  + apply H. eassumption.
+  + apply H0. assumption.
+- subst. eapply wAppLam.
+  + eapply H. eassumption.
+  + eapply H0. eassumption.
+  + eapply H1. eassumption.
+- subst. injection H2. intros. rewrite <- H3. eapply wAppInd.
+  + eapply H. eassumption.
+  + eapply H0. eassumption.
+  + eapply H1. eassumption.
+- subst. injection H2. intros. rewrite <- H3. eapply wAppCnstr.
+  + eapply H. eassumption.
+  + eapply H0. eassumption.
+  + eapply H1. eassumption.
+- subst. eapply wAppFix.
+  + apply H. eassumption.
+  + eassumption.
+  + apply H0. eassumption.
+- subst. eapply wConst. apply lookupDfn_LookupDfn. eassumption.
+  + apply H. eassumption.
+- subst. eapply wCasen; try eassumption.
+  + apply H. eassumption.
+  + apply H0. eassumption.
+- subst. eapply wCase0; try assumption.
+  + apply H. eassumption.
+  + eassumption.
+  + apply H0. eassumption.
+- subst. injection H1. intros. rewrite <- H2. constructor.
+  + apply H. assumption.
+  + apply H0. assumption.
+Qed.
+***)
+
+(* need this strengthening to large-enough fuel to make the induction
+** go through
+*)
+Lemma WcbvEval_wcbvEval:
+  forall p,
+    (forall t s, WcbvEval p t s ->
+             exists n, forall m, m >= n -> wcbvEval (S m) p t = Ret s) /\
+    (forall ts ss, WcbvEvals p ts ss ->
+             exists n, forall m, m >= n -> wcbvEvals (S m) p ts = Ret ss).
+intros p.
+assert (j:forall m x, m > x -> m = S (m - 1)). induction m; intuition.
+apply WcbvEvalEvals_ind; intros; try (exists 0; intros mx h; reflexivity).
+- destruct H. exists (S x). intros m hm. simpl. rewrite (j m x); try omega.
+  + rewrite (H (m - 1)); try omega. reflexivity. 
+- destruct H. exists (S x). intros m hm. simpl. rewrite (j m x); try omega.
+  + rewrite (H (m - 1)); try omega. reflexivity. 
+- destruct H. exists (S x). intros m h. simpl.
+  rewrite (j m x); try omega. apply H. omega.
+- destruct H. exists (S x).
+  assert (k:= LookupDfn_lookupDfn). intros m h. simpl.
+  erewrite k. rewrite (j m x). apply H. omega. omega.
+  eassumption. reflexivity.
+- destruct H, H0, H1. exists (S (max x (max x0 x1))). intros m h.
+  assert (k:wcbvEval m p fn = Ret (TLambda nm ty bod)).
+  + rewrite (j m (max x (max x0 x1))). apply H.
+    assert (l:= max_fst x (max x0 x1)); omega. omega.
+  + assert (k0:wcbvEval m p a1 = Ret a1').
+    rewrite (j m (max x (max x0 x1))). apply H0. 
+    assert (l:= max_snd x (max x0 x1)). assert (l':= max_fst x0 x1).
+    omega. omega.
+    * simpl. rewrite k. rewrite k0.
+      rewrite (j m (max x (max x0 x1))). apply H1.
+      assert (l:= max_snd x (max x0 x1)). assert (l':= max_snd x0 x1).
+      omega. omega.
+- destruct H, H0. exists (S (max x x0)). intros m h. simpl.
+  assert (k:wcbvEval m p dfn = Ret dfn'). 
+  assert (l:= max_fst x x0).
+  rewrite (j m (max x x0)). apply H. omega. omega.
+  rewrite k.
+  assert (l:= max_snd x x0).
+  rewrite (j m x0). apply H0. omega. omega.
+- destruct H, H0. exists (S (max x x0)). intros mx h.
+  assert (l1:= max_fst x x0). assert (l2:= max_snd x x0).
+  simpl. rewrite (j mx x); try rewrite (H (mx - 1)); try omega.
+  rewrite e. apply H0. omega.
+- destruct H, H0, H1. exists (S (max x (max x0 x1))). intros mx h.
+  assert (j1:= max_fst x (max x0 x1)). 
+  assert (lx: mx > x). omega.
+  assert (j2:= max_snd x (max x0 x1)).
+  assert (j3:= max_fst x0 x1).
+  assert (lx0: mx > x0). omega.
+  assert (j4:= max_snd x0 x1).
+  assert (j5:= max_fst x0 x1).
+  assert (lx1: mx > x1). omega.
+  simpl. rewrite (j mx x); try omega.
+  rewrite (H (mx - 1)); try omega.
+  rewrite (H0 (mx - 1)); try omega.
+  rewrite (H1 (mx - 1)); try omega. reflexivity.
+- destruct H, H0, H1. exists (S (max x (max x0 x1))). intros mx h.
+  assert (j1:= max_fst x (max x0 x1)). 
+  assert (lx: mx > x). omega.
+  assert (j2:= max_snd x (max x0 x1)).
+  assert (j3:= max_fst x0 x1).
+  assert (lx0: mx > x0). omega.
+  assert (j4:= max_snd x0 x1).
+  assert (j5:= max_fst x0 x1).
+  assert (lx1: mx > x1). omega.
+  simpl. rewrite (j mx x); try omega.
+  rewrite (H (mx - 1)); try omega.
+  rewrite (H0 (mx - 1)); try omega.
+  rewrite (H1 (mx - 1)); try omega. reflexivity.
+- destruct H, H0. exists (S (max x x0)). intros mx h.
+  assert (l1:= max_fst x x0). assert (l2:= max_snd x x0).
+  simpl. rewrite (j mx x); try rewrite (H (mx - 1)); try omega.
+  rewrite e. apply H0. omega.
+- destruct H, H0. exists (S (max x x0)). intros mx h.
+  assert (l1:= max_fst x x0). assert (l2:= max_snd x x0).
+  simpl. rewrite (j mx x); try rewrite (H (mx - 1)); try omega.
+  rewrite e. rewrite e0. apply H0. omega.
+- destruct H, H0. exists (S (max x x0)). intros m h.
+  assert (k:wcbvEval m p t = Ret t').
+  assert (l:= max_fst x x0).
+  rewrite (j m (max x x0)). apply H. omega. omega.
+  assert (k0:wcbvEvals m p ts = Ret ts').
+  assert (l:= max_snd x x0).
+  rewrite (j m (max x x0)). apply H0. omega. omega.
+  simpl. rewrite k. rewrite k0. reflexivity.
+Qed.
+
+Lemma WcbvEval_single_valued:
+  forall p t s, WcbvEval p t s -> forall u, WcbvEval p t u -> s = u.
+Proof.
+  intros p t s h0 u h1.
+  assert (j0:= proj1 (WcbvEval_wcbvEval _) _ _ h0).
+  assert (j1:= proj1 (WcbvEval_wcbvEval _) _ _ h1).
+  destruct j0 as [x0 k0].
+  destruct j1 as [x1 k1].
+  assert (l0:= k0 (max x0 x1) (max_fst x0 x1)).
+  assert (l1:= k1 (max x0 x1) (max_snd x0 x1)).
+  rewrite l0 in l1. injection l1. intuition.
+Qed.
+
+
+
+(**** scratch below here ****
+(** wcbvEval is monotonic in fuel **)
+Goal
+  forall t n p,  wcbvEval n p t = Some s ->
+                   wcbvEval n p t = wcbvEval (S n) p t.
+induction t; intros. 
+- destruct n0; simpl in H; intuition.
+- destruct n; simpl in H. intuition. reflexivity.
+- destruct n. simpl in H. intuition.  simpl in H. simpl.
+  change (TCast (wcbvEval n p t1) c t2 = TCast (wcbvEval (S n) p t1) c t2).
+  rewrite IHt1. reflexivity. intros h. rewrite <- h in H.
+
+unfold wcbvEval in H. simpl.
+
+
+         (forall (t s:Term), wcbvEval p t s ->
+             exists n, s = wcbvEval n p t) /\
+         (forall ts ss, WcbvEvals p ts ss ->
+             exists n, ss = tmap (wcbvEval n p) ts).
+Goal
+  forall (p:environ),
+         (forall (t s:Term), wcbvEval p t s ->
+             exists n, s = wcbvEval n p t) /\
+         (forall ts ss, WcbvEvals p ts ss ->
+             exists n, ss = tmap (wcbvEval n p) ts).
+
+(** WcbvEval and wcbvEval are the same relation **)
+Goal
+  forall (p:environ),
+         (forall (t s:Term), WcbvEval p t s ->
+             exists n, s = wcbvEval n p t) /\
+         (forall ts ss, WcbvEvals p ts ss ->
+             exists n, ss = tmap (wcbvEval n p) ts).
+intros p.
+apply WcbvEvalEvals_ind; intros; try (exists 1; reflexivity).
+- destruct H. exists (S x). subst.
+  assert (j:= proj2 (lookupDfn_LookupDfn _ _ _) l).
+  simpl. rewrite j. reflexivity.
+- destruct H. destruct H0. destruct H1.
+  exists (S (x + x0 + x1)). subst. unfold whBetaStep. simpl.
+
+
+
+Qed.
+
+
+(** If wcbvEval has fuel left, then it has reached a weak normal form **)
+(**
+Goal
+  forall (p:environ) t s n m, (wcbvEval n p t) = (S m, s) -> WNorm s.
+***)
+
+
+(***** scratch below here ****************
+
+
+Goal forall (p:environ) t s, WcbvEval p t s -> crct p t -> wNorm s = true.
+induction 1; destruct 1. 
+- apply IHWcbvEval. split. assumption. unfold weaklyClosed. intros nmx j.
+  unfold weaklyClosed in H2. apply H2. inversion H1. subst.
+  + specialize (H2 nm). unfold poccTrm in H2; simpl in H2.
+    rewrite string_eq_bool_rfl in H2. intuition.
+  + apply sBeta.
+
+
+
+HERE
+
+  + destruct (string_dec nmx nm).
+    * subst. unfold poccTrm. rewrite string_eq_bool_rfl. reflexivity.
+    * inversion H1. subst. inversion_clear H0. inversion H.
+  
+    simpl in H3.
+
+  + unfold poccTrm. inversion H1. subst. inversion h. unfold weaklyClosed in H3.
+    simpl in H3.
+
+
+
+
+Goal forall (p:environ), 
+  (forall t s, WcbvEval p t s -> crct p t -> wNorm s = true) /\
+  (forall ts ss, WcbvEvals p ts ss ->
+        Forall (crct p) ts -> Forall (fun s => wNorm s = true) ss).
+intros p.
+apply WcbvEvalEvals_ind.
+- intros nm t s q h1 h2 h3 h4. apply h3. inversion h2; subst.
+  + split.
+    * inversion h4. auto.
+    * unfold  weaklyClosed. intros nm1 j1.
+      simpl in j1. assert (j2:= string_eq_bool_eq _ _ j1). subst.
+      assert (j3:= proj2 (lookupDFN_LookupDFN _ _ _) H).
+      unfold lookupDfn. rewrite j3. intros j4. discriminate.
+  + destruct h4. split. auto. unfold weaklyClosed.
+    intros nm1 h4. simpl in h4.
+
+induction 1; inversion 1.
+- subst. elim (ncrct_nil_TConst nm _ _ H1); reflexivity.
+- subst. apply IHWcbvEval.
+
+HERE
+
+
+
+
+(***
+Lemma instantiate_arg_resp_WcbvEval:
+  (forall p ia2 s, WcbvEval p ia2 s -> 
+    forall a1 a2 bod, ia2 = (instantiate 0 bod a2) -> 
+    WcbvEval p a1 a2 -> WcbvEval p (instantiate 0 bod a1) s) /\
+  (forall p ia2 s, WcbvEvals p ia2s ss -> 
+    forall a1 a2 bod, ia2 = (instantiate 0 bod a2) -> 
+    WcbvEval p a1 a2 -> WcbvEval p (instantiate 0 bod a1) s)
+induction 1. intros ax a2 bod heq h.
+- eapply IHWcbvEval. intuition. assumption.
+- eapply IHWcbvEval3. assumption.
+- eapply IHWcbvEval2. assumption.
+- eapply 
+***)
+
+Lemma nat_compare_Gt: forall n, nat_compare (S n) n = Gt.
+induction n; intuition.
+Qed.
+Lemma nat_compare_Lt: forall n, nat_compare n (S n) = Lt.
+induction n; intuition.
+Qed.
+Lemma nat_compare_Eq: forall n, nat_compare n n = Eq.
+induction n; intuition.
+Qed.
+
+
+(**
+Goal
+  forall p ia2 s, WcbvEval p ia2 s -> 
+     forall bod a1 a2, ia2 = (instantiate 0 bod a2) -> WcbvEval p a1 a2 ->
+                    WcbvEval p (instantiate 0 bod a1) s.
+induction 1; intros bodx ax a2 heq h.
+- symmetry in heq. case (instantiate_is_Const _ _ _ _ heq); intro j.
+
+Lemma WcbvEval_unique:
+  forall (p:environ) (t s1:Term),
+    WcbvEval p t s1 -> forall (s2:Term), WcbvEval p t s2 -> s1 = s2.
+induction 1.
+- inversion_clear 1. eapply IHWcbvEval.
+  assert (j: t = t0). rewrite H in H2; injection H2; intuition.
+  rewrite j; assumption.
+- inversion_clear 1.
+  + eapply IHWcbvEval3. unfold whBetaStep. unfold whBetaStep in H5.
+    injection (IHWcbvEval1 _ H3); intros; subst.
+***)
+
+
+
+(**
+Ltac Tran_step := eapply Relation_Operators.rt1n_trans.
+
+Ltac const_step :=
+  tran_step; [eapply sConst; unfold lookupDfn, lookupDFN; simpl; reflexivity|].
+**)
+(***
+Goal
+  forall p fn nm ty bod a1 a1' s args,
+    clos_trans_n1 Term (wndEval p) fn (TLambda nm ty bod) ->
+    clos_trans_n1 Term (wndEval p) a1 a1' ->
+    clos_trans_n1 Term (wndEval p) (whBetaStep nm bod a1' args) s ->
+    clos_trans_n1 Term (wndEval p) (TApp fn (a1 :: args)) s.
+intros p fn nm ty bod a1 a1' s args hfn ha1 hstep.
+inversion hfn; inversion ha1; inversion hstep.
+- tran_step. eassumption.
+  tran_step. eapply sAppArgs. eapply saHd. eassumption.    
+  tran_step. eapply sBeta. eassumption.
+- tran_step. eapply sAppFun. eassumption.
+  tran_step. eapply sAppArgs. eapply saHd. eassumption.
+  tran_step. eapply sBeta. eassumption.
+- tran_step. eapply sAppFun. eassumption.
+  tran_step. eapply sAppArgs. eapply saHd. eapply tn1_step. eassumption.
+  tran_step. eapply sBeta. eassumption.
+***)
+
+
+(**
+Goal
+  forall p a a',
+    clos_refl_trans Term (wndEval p) a a' ->
+    forall bod args,
+      clos_refl_trans Term (wndEval p) (mkApp (instantiate 0 bod a) args)
+                         (mkApp (instantiate 0 bod a') args).
+intros p a a' h bod. induction h; intro args.
+- apply rt_step.
+ Check  Relation_Operators.rt1n_trans.
+
+
+
+Goal
+  forall p fn nm ty bod a1 a1' s args,
+    clos_refl_trans_1n Term (wndEval p) fn (TLambda nm ty bod) ->
+    clos_refl_trans_1n Term (wndEval p) a1 a1' ->
+    clos_refl_trans_1n Term (wndEval p) (whBetaStep nm bod a1' args) s ->
+    clos_refl_trans_1n Term (wndEval p) (TApp fn (a1 :: args)) s.
+intros p fn nm ty bod a1 a1' s args hfn ha1 hstep.
+inversion hfn; inversion ha1; inversion hstep.
+- tran_step. subst. eapply sBeta. subst. auto. 
+- tran_step. subst. eapply sBeta. subst. eassumption.
+- assert (j: clos_refl_trans_1n Term (wndEval p) a1 a1').
+  tran_step; eassumption.
+  tran_step. eapply sBeta. rewrite H3. destruct nm.
+  + simpl. simpl in H3. rewrite H3. eapply rt1n_refl.
+  + simpl. simpl in H3. rewrite <- H3.
+-
+
+
+ tran_step. eapply sAppArgs. eapply saHd. eassumption.
+  tran_step.
+
+  eapply (t1n_trans _ (wndEval p)). eapply t1n_step. eapply sAppArgs. eapply saHd.
+  eapply clos_t1n_trans. 
+
+eapply (t1n_trans _ (wndEval p)).
+
+
+ Check (t1n_trans _ _ _ H1).
+  tran_step. eapply sAppArgs. eapply saHd. eassumption.
+  tran_step. eapply sBeta. eassumption.
+- tran_step. eapply sAppFun. eassumption.
+
+
+Goal
+  forall p fn nm ty bod a1 a1' s args,
+    clos_trans_1n Term (wndEval p) fn (TLambda nm ty bod) ->
+    clos_trans_1n Term (wndEval p) a1 a1' ->
+    clos_trans_1n Term (wndEval p) (whBetaStep nm bod a1' args) s ->
+    clos_trans_1n Term (wndEval p) (TApp fn (a1 :: args)) s.
+intros p fn nm ty bod a1 a1' s args hfn ha1 hstep.
+inversion hfn; inversion ha1; inversion hstep.
+- tran_step. eapply sAppFun. eassumption.
+  tran_step. eapply sAppArgs. eapply saHd. eassumption.    
+  tran_step. eapply sBeta. eassumption.
+- tran_step. eapply sAppFun. eassumption.
+  tran_step. eapply sAppArgs. eapply saHd. eassumption.
+  tran_step. eapply sBeta. eassumption.
+- tran_step. eapply sAppFun. eassumption.
+
+  tran_step. eapply sAppArgs. eapply saHd. eassumption.
+  tran_step. eapply sBeta. eassumption.
+
+
+Goal
+  forall p fn nm ty bod a1 a1' s args,
+    clos_trans Term (wndEval p) fn (TLambda nm ty bod) ->
+    clos_trans Term (wndEval p) a1 a1' ->
+    clos_trans Term (wndEval p) (whBetaStep nm bod a1' args) s ->
+    clos_trans Term (wndEval p) (TApp fn (a1 :: args)) s.
+intros p fn nm ty bod a1 a1' s args hfn ha1 hstep.
+inversion hfn; inversion ha1; inversion hstep.
+- tran_step. eapply sAppFun. eassumption.
+  tran_step. eapply sAppArgs. eapply saHd. eassumption.    
+  tran_step. eapply sBeta.
+  eassumption.
+unfold whBetaStep in H3.
+***)
+
+(**
+Ltac Tran_step := eapply Relation_Operators.rt1n_trans.
+
+Goal forall p t t', WcbvEval p t t' -> clos_refl_trans_1n _ (wndEval p) t t'.
+induction 1.
+- Tran_step. eapply sConst. rewrite H. reflexivity. assumption.
+- tran_step. eapply sAppFun.
+Check (rt_refl Term (wndEval p)). _ (wndEval p) _ IHWcbvEval1).
+**)
+
+(** use a timer to make this Terminate **)
+Fixpoint wcbvEval (tmr:nat) (p:environ) (t:Term) {struct tmr} : nat * Term :=
+  match tmr with 
+    | 0 => (0, t)          (** out of time  **)
+    | S n => match t with  (** look for a redex **)
+               | TConst nm => match (lookupDfn nm p) with
+                                | Some t => wcbvEval n p t
+                                | None =>  (0, TUnknown nm)
+                              end
+               | TApp fn (cons a1 args) =>
+                 let efn := snd (wcbvEval n p fn) in
+                 match efn with
+                   | TLambda _ _ bod =>
+                     let wharg := snd (wcbvEval n p a1) in
+                     wcbvEval n p (whBetaStep bod wharg args)
+                   | TFix dts m => wcbvEval n p (whFixStep dts m args)
+                   | TConstruct _ r =>
+                     let eargs := map (compose (@snd nat Term) (wcbvEval n p))
+                                      (cons a1 args) in
+                     (n, mkApp efn eargs)
+                   | _ => (n, TUnknown"App")
+                 end
+               | TCase np _ mch brs =>
+                 match evCanon n p mch with
+                   | Some (cstr, args) =>
+                     wcbvEval n p (whCaseStep cstr (skipn np args) brs)
+                   | None => (n, mch)
+                 end
+               | TLetIn nm df ty bod =>
+                 wcbvEval n p (TApp (TLambda nm ty bod) (df::nil))
+               | TCast t1 ck t2 => (n, TCast (snd (wcbvEval n p t1)) ck t2)
+               (** already in whnf ***)
+               | TLambda nn ty t => (n, TLambda nn ty t)
+               | TProd nn ty t => (n, TProd nn ty t)
+               | TFix mfp br => (n, TFix mfp br)
+               | TConstruct i cn => (n, TConstruct i cn)
+               | TInd i => (n, TInd i)
+               | TSort => (n, TSort)
+               (** should never appear **)
+               | TApp _ nil => (0, TUnknown "App no args")
+               | TRel _ => (0, TUnknown "TRel")
+               | TUnknown s => (0, TUnknown s)
+             end
+  end
+(***
+with
+wcbvEvalArgs tmr p (ts:Terms) {struct ts} : Terms :=
+  match ts with
+    | nil => nil
+    | cons t ts => cons (snd (wcbvEval tmr p t)) (wcbvEvalArgs tmr p ts)
+  end
+***)
+with evCanon tmr p (t:Term) {struct tmr} : option (nat * Terms) :=
+  match tmr with
+    | 0 => None              (** out of time  **)
+    | S n => match (wcbvEval n p t) with
+               | (_, TConstruct _ cstr) => Some (cstr, nil)
+               | (_, TApp (TConstruct _ cstr) ts) => Some (cstr, ts)
+               | x => None
+             end
+  end.
+
+
+Definition Nat := nat.
+Definition typedef := ((fun (A:Type) (a:A) => a) Nat 1).
+Quote Definition q_typedef := Eval compute in typedef.
+Quote Recursively Definition p_typedef := typedef.
+Definition P_typedef := program_Program p_typedef nil.
+Definition Q_typedef := 
+  Eval compute in (wcbvEval 100 (env P_typedef) (main P_typedef)).
+Goal snd Q_typedef = q_typedef.
+reflexivity.
+Qed.
+
+
+Definition II := fun (A:Type) (a:A) => a.
+Quote Definition q_II := Eval compute in II.
+Quote Recursively Definition p_II := II.
+Definition P_II := program_Program p_II nil.
+Definition Q_II :=
+  Eval compute in (wcbvEval 4 (env P_II)) (main P_II).
+Goal snd Q_II = q_II.
+reflexivity.
+Qed.
+
+(***
+Eval cbv in (wcbvEval 4 p_II) (main p_II).
+Quote Recursively Definition II_nat_pgm := (II nat).
+Print II_nat_pgm.
+Eval compute in (wcbvEval 4 II_nat_pgm) (main II_nat_pgm).
+
+
+Quote Definition II_2_Term := (II nat 2).
+Print II_2_Term.
+Eval compute in II_2_Term.
+Quote Recursively Definition II_2_program := (II nat 2).
+Print II_2_program.
+Quote Definition two_Term := 2.
+
+Eval cbv in (wcbvEval 4 II_2_program) (main II_2_program).
+
+Quote Recursively Definition p_plus22 := (plus 2 2).
+Print p_plus22.
+Quote Definition q_ans := 4.
+Eval cbv in (wcbvEval 20 p_plus22) (main p_plus22).
+
+Eval compute in (plus 1 2).
+Quote Recursively Definition p_plus12 := (plus 1 2).
+Eval cbv in (wcbvEval 99 p_plus12) (main p_plus12).
+
+Quote Recursively Definition p_anon := ((fun (_:nat) => 1 + 3) (3 * 3)).
+Eval cbv in (wcbvEval 20 p_anon) (main p_anon).
+
+Fixpoint even (n:nat) : bool :=
+  match n with
+    | 0 => true
+    | (S n) => odd n
+  end
+with
+odd (n:nat) : bool :=
+  match n with
+    | 0 => false
+    | (S n) => even n
+  end.
+
+Quote Recursively Definition p_even99 := (even 99).
+Time Eval cbv in (wcbvEval 500 p_even99) (main p_even99).
+Quote Recursively Definition p_odd99 := (odd 99).
+Time Eval cbv in (wcbvEval 500 p_odd99) (main p_odd99).
+
+
+Fixpoint slowFib (n:nat) : nat :=
+  match n with
+    | 0 => 0
+    | S m => match m with
+               | 0 => 1
+               | S p => slowFib p + slowFib m
+             end
+  end.
+Eval compute in (slowFib 0).
+Eval compute in (slowFib 1).
+Eval compute in (slowFib 2).
+Eval compute in (slowFib 3).
+Eval compute in (slowFib 4).
+Quote Recursively Definition p_slowFib1 := (slowFib 1).
+Quote Recursively Definition p_slowFib2 := (slowFib 2).
+Quote Recursively Definition p_slowFib3 := (slowFib 3).
+Quote Recursively Definition p_slowFib4 := (slowFib 4).
+Quote Recursively Definition p_slowFib5 := (slowFib 5).
+Quote Recursively Definition p_slowFib6 := (slowFib 6).
+Quote Recursively Definition p_slowFib7 := (slowFib 7).
+Quote Recursively Definition p_slowFib10 := (slowFib 10).
+Quote Recursively Definition p_slowFib15 := (slowFib 15).
+Eval cbv in (wcbvEval 99 p_slowFib3) (main p_slowFib3).
+Eval cbv in (wcbvEval 99 p_slowFib4) (main p_slowFib4).
+Eval cbv in (wcbvEval 99 p_slowFib5) (main p_slowFib5).
+Eval cbv in (wcbvEval 99 p_slowFib6) (main p_slowFib6).
+Time Eval cbv in (wcbvEval 99 p_slowFib7) (main p_slowFib7).
+Time Eval cbv in (wcbvEval 99 p_slowFib10) (main p_slowFib10).
+Time Eval cbv in (wcbvEval 200 p_slowFib15) (main p_slowFib15).
+
+
+Fixpoint fibrec (n:nat) (fs:nat * nat) {struct n} : nat :=
+  match n with
+    | 0 => fst fs
+    | (S n) => fibrec n (pair ((fst fs) + (snd fs)) (fst fs))
+  end.
+Definition fib : nat -> nat := fun n => fibrec n (pair 0 1).
+
+Eval compute in (fib 0).
+Eval compute in (fib 1).
+Eval compute in (fib 2).
+Eval compute in (fib 3).
+Eval compute in (fib 4).
+Eval compute in (fib 6).
+Quote Recursively Definition p_fib1 := (fib 1).
+Quote Recursively Definition p_fib2 := (fib 2).
+Quote Recursively Definition p_fib3 := (fib 3).
+Quote Recursively Definition p_fib4 := (fib 4).
+Quote Recursively Definition p_fib5 := (fib 5).
+Quote Recursively Definition p_fib6 := (fib 6).
+Quote Recursively Definition p_fib7 := (fib 7).
+Quote Recursively Definition p_fib10 := (fib 10).
+Quote Recursively Definition p_fib15 := (fib 15).
+Eval cbv in (wcbvEval 20 p_fib1) (main p_fib1).
+Eval cbv in (wcbvEval 30 p_fib2) (main p_fib2).
+Eval cbv in (wcbvEval 40 p_fib3) (main p_fib3).
+Eval cbv in (wcbvEval 50 p_fib4) (main p_fib4).
+Eval cbv in (wcbvEval 60 p_fib5) (main p_fib5).
+Eval cbv in (wcbvEval 60 p_fib6) (main p_fib6).
+Time Eval cbv in (wcbvEval 70 p_fib7) (main p_fib7).
+Time Eval cbv in (wcbvEval 70 p_fib10) (main p_fib10).
+Time Eval cbv in (wcbvEval 200 p_fib15) (main p_fib15).
+
+
+Quote Recursively Definition l_fib4 := (let x := 4 in fib x).
+Eval cbv in (wcbvEval 50 l_fib4) (main l_fib4).
+
+Fixpoint evenP (n:nat) {struct n} : bool :=
+  match n with
+    | 0 => true
+    | S p => (oddP p)
+  end
+with oddP (n:nat) : bool :=
+  match n with
+    | 0 => false
+    | S p => evenP p
+  end.
+
+Quote Recursively Definition p_evenOdd := (even 100).
+Quote Recursively Definition f_evenOdd := (odd 100).
+Eval cbv in (wcbvEval 500 p_evenOdd) (main p_evenOdd).
+Eval cbv in (wcbvEval 500 f_evenOdd) (main f_evenOdd).
+
+Quote Recursively Definition l_evenOdd := (even (let x := 50 in 2 * x)).
+Time Eval cbv in (wcbvEval 500 l_evenOdd) (main l_evenOdd).
+Time Eval cbv in (wcbvEval 5000 l_evenOdd) (main l_evenOdd).
+
+Parameter axiom:nat.
+Quote Recursively Definition p_axiom := (let x := axiom in 2 * x).
+Print p_axiom.
+Time Eval cbv in (wcbvEval 100 p_axiom) (main p_axiom).
+Time Eval cbv in (wcbvEval 200 p_axiom) (main p_axiom).
+
+***********)
+
+(***
+Goal forall p s t,
+       WcbvEval p s t -> exists (n m:nat), wcbvEval n p s  = (S m, t).
+induction 1.
+- destruct IHWcbvEval. destruct H1. exists (S x). exists x0.
+  simpl. rewrite H. assumption.
+- destruct IHWcbvEval1, IHWcbvEval2, IHWcbvEval3.
+  destruct H2, H3, H4.
+  exists (S (x + x0 + x1)). exists (S (x2 + x3 + x4)).
+  simpl.
+***)
+
+(* Coq doesn't evaluate the type of a cast *)
+Eval cbv in  3 : ((fun n:Type => nat) Prop).
+Eval lazy in  3 : ((fun n:Type => nat) Prop).
+Eval hnf in  3 : ((fun n:Type => nat) Prop).
+Eval vm_compute in  3 : ((fun n:Type => nat) Prop).
+
+Goal 
+  forall (t s:Term) (n m:nat) (e:environ),
+  wcbvEval (S n) e t = (S m,s) -> wNorm s = true.
+intros t; induction t; intros; try discriminate;
+try (injection H; intros h1 h2; rewrite <- h1; auto; subst).
+- simpl. simpl in H. rewrite h2 in H. rewrite h1. erewrite IHt1.
+
+
+Lemma not_ltb_n_0: forall (n:nat), ltb n 0 = false.
+induction n; unfold ltb; reflexivity.
+Qed.
+
+Lemma wcbvEval_up:
+  forall (n:nat) (p:program) (s:Term),
+   closedTerm 0 s = true -> fst (wcbvEval n p s) > 0 ->
+   snd (wcbvEval n p s) = snd (wcbvEval (S n) p s).
+intros n p s h1. induction n. simpl. omega.
+intros h2.
+induction s; simpl in h1; try rewrite not_ltb_n_0 in h1;
+try discriminate; try reflexivity.
+Admitted.
+
+(***
+intros n p s h. induction n. simpl. intro h1. omega.
+intro h1. induction s; try reflexivity.
+- rewrite IHs2.
+***)
+
+Goal forall (strt:nat) (p:program) (s:Term),
+       wNorm s = true -> snd (wcbvEval strt p s) = s.
+intros strt p s h. induction strt. reflexivity.
+induction s; simpl in h; try discriminate h; try reflexivity.
+- rewrite <- IHstrt. rewrite -> IHstrt at 1. rewrite <- wcbvEval_up. reflexivity. simpl.
+
+- rewrite <- IHstrt. rewrite -> IHstrt at 1. admit.
+- rewrite <- IHstrt. rewrite -> IHstrt at 1. admit.
+- rewrite <- IHstrt. rewrite -> IHstrt at 1. admit.
+- rewrite <- IHstrt. rewrite -> IHstrt at 1. admit.
+Qed.
+
+Goal forall (strt:nat) (p:program) (s:Term),
+       fst (wcbvEval strt p s) > 0 -> wNorm (snd (wcbvEval strt p s)) = true.
+intros strt p s h. induction s; unfold wcbvEval; simpl.
+
+*******************)
+*****)
