Randy_8.5beta2/RandyWorking/L2_typeStrippedL1/stripEvalCommute.v
@@ -1,0 +1,1120 @@
+Add LoadPath "../common" as Common.
+Add LoadPath "../L1_MalechaQuoted" as L1.
+Add LoadPath "." as L2.
+
+Require Import Lists.List.
+Require Import Strings.String.
+Require Import Strings.Ascii.
+Require Import Arith.Compare_dec.
+Require Import Arith.Peano_dec.
+Require Import Setoid.
+Require L1.L1.
+Require Import L2.term.
+Require Import L2.program.
+Require Import L2.wndEval.
+Require Import L2.wcbvEval.
+
+Local Open Scope string_scope.
+Local Open Scope bool.
+Local Open Scope list.
+Set Implicit Arguments.
+
+Definition L1Term := L1.term.Term.
+Definition L1Terms := L1.term.Terms.
+Definition L1Defs := L1.term.Defs.
+
+Function strip (t:L1Term) : Term :=
+  match t with
+    | L1.term.TRel n => TRel n
+    | L1.term.TSort s => TSort s
+    | L1.term.TCast t _ _ => TCast (strip t)
+    | L1.term.TProd nm _ bod => TProd nm (strip bod)
+    | L1.term.TLambda nm _ bod => TLambda nm (strip bod)
+    | L1.term.TLetIn nm dfn _ bod => TLetIn nm (strip dfn) (strip bod)
+    | L1.term.TApp fn arg args => TApp (strip fn) (strip arg) (strips args)
+    | L1.term.TConst nm => TConst nm
+    | L1.term.TInd i => TInd i
+    | L1.term.TConstruct i m => TConstruct i m
+    | L1.term.TCase n _ mch brs => TCase n (strip mch) (strips brs)
+    | L1.term.TFix ds n => TFix (stripDs ds) n
+  end
+with strips (ts:L1Terms) : Terms := 
+  match ts with
+    | L1.term.tnil => tnil
+    | L1.term.tcons t ts => tcons (strip t) (strips ts)
+  end
+with stripDs (ts:L1Defs) : Defs := 
+  match ts with
+    | L1.term.dnil => dnil
+    | L1.term.dcons nm _ t m ds => dcons nm (strip t) m (stripDs ds)
+  end.
+
+(*** ???
+Lemma strip_absorbs_mkApp_nil:
+  forall t, mkApp (strip t) tnil = strip t.
+induction t; simpl; try reflexivity.
+- rewrite tappend_tnil. reflexivity.
+Qed.
+Hint Resolve strip_absorbs_mkApp_nil.
+****)
+
+
+Definition optStrip (t:option L1Term) : option Term :=
+  match t with
+    | None => None
+    | Some t => Some (strip t)
+  end.
+Definition optStrips (ts:option L1Terms) : option Terms :=
+  match ts with
+    | None => None
+    | Some ts => Some (strips ts)
+  end.
+
+Lemma optStrip_hom: forall y, optStrip (Some y) = Some (strip y).
+induction y; simpl; reflexivity.
+Qed.
+Lemma optStrips_hom: forall y, optStrips (Some y) = Some (strips y).
+induction y; simpl; reflexivity.
+Qed.
+
+Function stripCnstrs (cs:list L1.program.Cnstr) : list Cnstr :=
+  match cs with
+    | nil => nil
+    | cons (L1.program.mkCnstr str arity) cs =>
+        cons (mkCnstr str arity) (stripCnstrs cs)
+  end.
+Function stripItyPack (its:L1.program.itypPack) : L2.program.itypPack :=
+  match its with
+    | nil => nil
+    | (L1.program.mkItyp str itps) :: itpacks =>
+         (L2.program.mkItyp str (stripCnstrs itps)) ::
+                           stripItyPack itpacks
+  end.
+Function stripEc (ec:L1.program.envClass) : L2.program.envClass :=
+  match ec with
+    | L1.program.ecTrm t => L2.program.ecTrm (strip t)
+    | L1.program.ecTyp itp => L2.program.ecTyp (stripItyPack itp)
+  end.
+
+Fixpoint stripEnv (p:L1.program.environ) : environ :=
+  match p with
+    | nil => nil
+    | cons (nm, ec) q => cons (nm, (stripEc ec)) (stripEnv q)
+  end.
+
+Definition program_Program (pgm:program) : option Program :=
+  match L1.malecha_L1.program_Program pgm (ret nil) with
+    | Exc str => None
+    | Ret pgm => Some {| env:= stripEnv (L1.program.env pgm);
+                         main:= strip (L1.program.main pgm) |}
+  end.
+Definition term_Term (t:term) : option Term :=
+  match L1.malecha_L1.term_Term t with
+    | Exc str => None
+    | Ret trm => Some (strip trm)
+  end.
+
+Lemma stripEnv_hom:
+  forall str (ec:L1.program.envClass) p,
+    stripEnv ((str, ec) :: p) = (str, (stripEc ec))::(stripEnv p).
+induction p; destruct ec; try reflexivity.
+Qed.
+
+Lemma Lookup_hom:
+ forall p s ec, L1.program.Lookup s p ec -> 
+               Lookup s (stripEnv p) (stripEc ec).
+induction 1; destruct t.
+- change (Lookup s ((s, L2.program.ecTrm (strip t)) :: (stripEnv p))
+                    (L2.program.ecTrm (strip t))).
+  apply L2.program.LHit.
+- change (Lookup s ((s, L2.program.ecTyp (stripItyPack i)) :: (stripEnv p))
+                    (L2.program.ecTyp (stripItyPack i))).
+  apply L2.program.LHit.
+- change (Lookup s2 ((s1, L2.program.ecTrm (strip t)) :: (stripEnv p))
+                     (stripEc ec)).
+  apply L2.program.LMiss; assumption.
+- change (Lookup s2 ((s1, L2.program.ecTyp (stripItyPack i)) :: (stripEnv p))
+                     (stripEc ec)).
+  apply L2.program.LMiss; assumption.
+Qed.
+
+Lemma LookupDfn_hom:
+ forall p s t, L1.program.LookupDfn s p t -> 
+               LookupDfn s (stripEnv p) (strip t).
+unfold L1.program.LookupDfn, L2.program.LookupDfn. intros.
+assert (j:= Lookup_hom H). exact j.
+Qed.
+
+Lemma dlength_hom:
+  forall ds, L1.term.dlength ds = dlength (stripDs ds).
+induction ds. intuition. simpl. rewrite IHds. reflexivity.
+Qed.
+
+Lemma tcons_hom:
+  forall t ts, strips (L1.term.tcons t ts) = tcons (strip t) (strips ts).
+reflexivity.
+Qed.
+
+Lemma tnil_hom: strips L1.term.tnil = tnil.
+reflexivity.
+Qed.
+
+Lemma dcons_hom:
+  forall nm ty bod rarg ds,
+    stripDs (L1.term.dcons nm ty bod rarg ds) =
+    dcons nm (strip bod) rarg (stripDs ds).
+reflexivity.
+Qed.
+
+Lemma dnil_hom: stripDs L1.term.dnil = dnil.
+reflexivity.
+Qed.
+
+Lemma dnthBody_hom:
+  forall m ds, optStrip (L1.term.dnthBody m ds) = dnthBody m (stripDs ds).
+induction m; induction ds; try intuition.
+- simpl. intuition.
+Qed.
+
+Lemma tnth_hom:
+ forall ts n, optStrip (L1.term.tnth n ts) = tnth n (strips ts).
+induction ts; simpl; intros n; case n; try reflexivity; trivial.
+Qed. 
+
+Lemma tskipn_hom:
+  forall ts n, optStrips (L1.term.tskipn n ts) = tskipn n (strips ts).
+induction ts; simpl; intros n; case n; try reflexivity; trivial.
+Qed.
+
+Lemma tappend_hom:
+  forall ts us,
+    strips (L1.term.tappend ts us) = tappend (strips ts) (strips us).
+induction ts; intros us; simpl. reflexivity.
+rewrite IHts. reflexivity.
+Qed.
+
+Lemma TApp_hom:
+  forall fn arg args,
+    strip (L1.term.TApp fn arg args) =
+    TApp (strip fn) (strip arg) (strips args).
+induction fn; intros arg args; try reflexivity.
+Qed.
+
+Lemma isApp_hom:
+  forall t, isApp (strip t) -> L1.term.isApp t.
+destruct t; simpl; intros h; destruct h as [x0 [x1 [x2 h]]]; try discriminate. 
+- exists t1, t2, t3. reflexivity.
+Qed.
+
+Lemma mkApp_tcons_lem1:
+  forall fn arg args,
+    mkApp (mkApp fn (tcons arg args)) tnil = mkApp fn (tcons arg args).
+Proof.
+  destruct fn; intros arg args; simpl;
+  try rewrite tappend_tnil; try reflexivity.
+Qed.
+
+Lemma mkApp_tcons_lem2:
+ forall fn ts u s args,
+   mkApp fn (tcons u (tappend ts (tcons s args))) =
+   mkApp (mkApp fn (tcons u ts)) (tcons s args).
+Proof.
+  destruct fn; destruct ts; intros; try reflexivity.
+  - rewrite mkApp_idempotent. simpl. reflexivity.
+  - rewrite mkApp_idempotent. simpl. reflexivity.
+Qed.
+
+Lemma mkApp_hom:
+forall fn args,
+  strip (L1.term.mkApp fn args) = mkApp (strip fn) (strips args).
+Proof.
+  induction fn; induction args; simpl; try reflexivity.
+  - rewrite tappend_tnil. rewrite L1.term.tappend_tnil. reflexivity.
+  - rewrite <- tcons_hom. rewrite <- tappend_hom. reflexivity.
+Qed.
+
+Lemma TCast_hom:
+  forall tm ck ty, strip (L1.term.TCast tm ck ty) = TCast (strip tm).
+reflexivity.
+Qed.
+
+Lemma instantiate_tappend_commute:
+  forall ts us tin n,
+    instantiates tin n (tappend ts us) =
+    tappend (instantiates tin n ts) (instantiates tin n us).
+induction ts; intros.
+- reflexivity.
+- change (tcons (instantiate tin n t) (instantiates tin n (tappend ts us)) =
+          tcons (instantiate tin n t) (tappend (instantiates tin n ts)
+                                               (instantiates tin n us))).
+ rewrite IHts. reflexivity.
+Qed.
+
+Lemma instantiates_tcons_commute:
+  forall tin n t ts,
+         (instantiates tin n (tcons t ts)) = 
+         (tcons (instantiate tin n t) (instantiates tin n ts)).
+intros tin n t ts. reflexivity.
+Qed.
+
+Lemma instantiate_mkApp_commute:
+forall tin n bod arg args,
+  instantiate tin n (mkApp bod (tcons arg args)) =
+  mkApp (instantiate tin n bod) (tcons (instantiate tin n arg)
+                                       (instantiates tin n args)).
+induction bod; simpl; intros; try reflexivity.
+- change
+    (mkApp (instantiate tin n bod1) 
+           (tcons (instantiate tin n bod2)
+                     (instantiates tin n (tappend t (tcons arg args)))) =
+     mkApp (mkApp (instantiate tin n bod1)
+                  (tcons (instantiate tin n bod2)
+                         (instantiates tin n t)))
+           (tcons (instantiate tin n arg) (instantiates tin n args))).
+  rewrite mkApp_idempotent. simpl. 
+  rewrite instantiate_tappend_commute. rewrite instantiates_tcons_commute.
+  reflexivity.
+Qed.
+
+Lemma instantiate_mkApp_nil_commute:
+forall tin n bod,
+  instantiate tin n (mkApp bod tnil) = mkApp (instantiate tin n bod) tnil.
+induction bod; simpl; intros; try reflexivity.
+- destruct (lt_eq_lt_dec n n0) as [[h1 | h2 ] | h3].
+  + unfold instantiate. rewrite (proj1 (nat_compare_lt _ _) h1). 
+    simpl. reflexivity.
+  + subst. unfold instantiate. rewrite (proj2 (nat_compare_eq_iff n0 n0)).
+    * rewrite mkApp_idempotent. simpl. reflexivity.
+    * reflexivity.
+  + unfold instantiate. rewrite (proj1 (nat_compare_gt _ _) h3).
+    simpl. reflexivity.
+- rewrite tappend_tnil.
+  change (instantiate tin n (TApp bod1 bod2 t) =
+         mkApp (mkApp (instantiate tin n bod1)
+                      (tcons (instantiate tin n bod2)
+                             (instantiates tin n t)))
+                      tnil).
+  rewrite mkApp_idempotent. simpl. rewrite tappend_tnil. reflexivity. 
+Qed.
+
+Lemma instantiate_hom:
+    (forall bod arg n, strip (L1.term.instantiate arg n bod) =
+                   instantiate (strip arg) n (strip bod)) /\
+    (forall bods arg n, strips (L1.term.instantiates arg n bods) =
+                    instantiates (strip arg) n (strips bods)) /\
+    (forall ds arg n, stripDs (L1.term.instantiateDefs arg n ds) =
+                    instantiateDefs (strip arg) n (stripDs ds)).
+apply L1.term.TrmTrmsDefs_ind; intros; try (simpl; reflexivity).
+- simpl. destruct (lt_eq_lt_dec n n0);
+         unfold L1.term.instantiate; unfold instantiate.
+  + destruct s.
+    * rewrite (proj1 (nat_compare_gt n0 n)); trivial.
+    * subst. rewrite (proj2 (nat_compare_eq_iff _ _)); trivial.
+      rewrite mkApp_hom. rewrite tnil_hom. reflexivity.
+  + rewrite (proj1 (nat_compare_lt n0 n)); trivial.
+- change (TCast (strip (L1.term.instantiate arg n t)) =
+         (TCast (instantiate (strip arg) n (strip t)))).
+  rewrite H. reflexivity.
+- change (TProd n (strip (L1.term.instantiate arg (S n0) t0)) =
+         (TProd n (instantiate (strip arg) (S n0) (strip t0)))).
+  rewrite H0. reflexivity.
+- change (TLambda n (strip (L1.term.instantiate arg (S n0) t0)) =
+         (TLambda n (instantiate (strip arg) (S n0) (strip t0)))).
+  rewrite H0. reflexivity.
+- change (TLetIn n (strip (L1.term.instantiate arg n0 t))
+                   (strip (L1.term.instantiate arg (S n0) t1)) =
+         (TLetIn n (instantiate (strip arg) n0 (strip t))
+                   (instantiate (strip arg) (S n0) (strip t1)))).
+  rewrite H. rewrite H1. reflexivity.
+- change (strip (L1.term.mkApp
+                   (L1.term.instantiate arg n t)
+                   (L1.term.tcons (L1.term.instantiate arg n t0)
+                                  (L1.term.instantiates arg n t1))) =
+          instantiate (strip arg) n (strip (L1.term.TApp t t0 t1))). 
+  rewrite TApp_hom. 
+  change
+    (strip (L1.term.mkApp (L1.term.instantiate arg n t)
+                          (L1.term.tcons (L1.term.instantiate arg n t0)
+                                         (L1.term.instantiates arg n t1))) =
+     (mkApp (instantiate (strip arg) n (strip t))
+            (tcons (instantiate (strip arg) n (strip t0))
+                   (instantiates (strip arg) n (strips t1))))).
+  rewrite <- H. rewrite <- H0. rewrite <- H1. 
+  rewrite mkApp_hom. rewrite tcons_hom. reflexivity. 
+- change (TCase n (strip (L1.term.instantiate arg n0 t0))
+                (strips (L1.term.instantiates arg n0 t1)) =
+         (TCase n (instantiate (strip arg) n0 (strip t0))
+                (instantiates (strip arg) n0 (strips t1)))).
+  rewrite H0. rewrite H1. reflexivity.
+- change (TFix (stripDs (L1.term.instantiateDefs arg
+                                              (n0 + L1.term.dlength d) d)) n =
+         (TFix (instantiateDefs (strip arg)
+                                (n0 + dlength (stripDs d)) (stripDs d)) n)).
+  rewrite H. rewrite dlength_hom. reflexivity.
+- change (tcons (strip (L1.term.instantiate arg n t))
+                (strips (L1.term.instantiates arg n t0)) =
+          tcons (instantiate (strip arg) n (strip t))
+                (instantiates (strip arg) n (strips t0))).
+  rewrite H. rewrite H0. reflexivity.
+- change (dcons n (strip (L1.term.instantiate arg n1 t0)) n0
+                  (stripDs (L1.term.instantiateDefs arg n1 d)) =
+          dcons n (instantiate (strip arg) n1 (strip t0)) n0
+                (instantiateDefs (strip arg) n1 (stripDs d))).
+  rewrite H0. rewrite H1. reflexivity.
+Qed.
+
+
+Lemma whBetaStep_hom:
+  forall bod arg args,
+    strip (L1.term.whBetaStep bod arg args) =
+    whBetaStep (strip bod) (strip arg) (strips args).
+intros bod arg args.
+unfold L1.term.whBetaStep, whBetaStep.
+rewrite mkApp_hom. rewrite <- (proj1 instantiate_hom). reflexivity.
+Qed.
+
+Lemma TConstruct_hom:  (****  WRONG: arity ****)
+  forall i n , strip (L1.term.TConstruct i n) = TConstruct i n.
+intros. simpl.  destruct i. reflexivity.
+Qed.
+
+
+Lemma optStrip_match:
+  forall x (f:L1Term -> L1Term) (g:Term -> Term), 
+    (forall z, strip (f z) = g (strip z)) ->
+    optStrip (match x with Some y => Some (f y) | None => None end) =
+    match (optStrip x) with Some y => Some (g y) | None => None end.
+induction x; intros f g h; simpl.
+- rewrite h; reflexivity.
+- reflexivity.
+Qed.
+
+Lemma whCaseStep_hom:
+  forall n brs ts,
+    optStrip (L1.term.whCaseStep n ts brs) =
+    whCaseStep n (strips ts) (strips brs).
+destruct n, brs; intros; simpl; try reflexivity.
+- unfold whCaseStep. simpl. rewrite mkApp_hom. reflexivity.
+- unfold whCaseStep. unfold L1.term.whCaseStep. simpl. 
+  rewrite <- tnth_hom. destruct (L1.term.tnth n brs); simpl.
+  + rewrite mkApp_hom. reflexivity.
+  + reflexivity.
+Qed.
+
+Lemma TFix_hom:
+  forall defs n, strip (L1.term.TFix defs n) = TFix (stripDs defs) n.
+reflexivity.
+Qed.
+
+Lemma TProd_hom:
+  forall nm ty bod, strip (L1.term.TProd nm ty bod) = TProd nm (strip bod).
+reflexivity.
+Qed.
+
+Lemma TLambda_hom:
+  forall nm ty bod, strip (L1.term.TLambda nm ty bod) = TLambda nm (strip bod).
+reflexivity.
+Qed.
+
+Lemma TLetIn_hom:
+  forall nm dfn ty bod,
+    strip (L1.term.TLetIn nm dfn ty bod) = TLetIn nm (strip dfn) (strip bod).
+reflexivity.
+Qed.
+
+Lemma TCase_hom:
+  forall n ty mch brs,
+    strip (L1.term.TCase n ty mch brs) = TCase n (strip mch) (strips brs).
+reflexivity.
+Qed.
+
+Lemma fold_left_hom:
+forall (F:L1Term -> nat -> L1Term) 
+       (stripF:Term -> nat -> Term) (ns:list nat) (t:L1Term),
+  (forall (s:L1Term) (n:nat), strip (F s n) = stripF (strip s) n) ->
+  strip (fold_left F ns t) = fold_left stripF ns (strip t).
+induction ns; intros t h.
+- intuition.
+- simpl. rewrite IHns.
+  + rewrite h. reflexivity.
+  + assumption.
+Qed.
+
+Lemma pre_whFixStep_hom:
+  forall body dts args,
+    pre_whFixStep (strip body) (stripDs dts) (strips args) =
+    strip (L1.term.pre_whFixStep body dts args).
+Proof.
+  intros body dts args.
+  destruct dts, args; unfold pre_whFixStep, L1.term.pre_whFixStep;
+  simpl; rewrite mkApp_hom; try reflexivity.
+  - rewrite (fold_left_hom _
+          (fun (bod : Term) (ndx : nat) =>
+                instantiate (TFix (dcons n (strip t0) n0 (stripDs dts)) ndx)
+                  0 bod)).
+    + rewrite <- (dcons_hom _ L1.term.prop). rewrite (proj1 instantiate_hom).
+      rewrite <- dlength_hom. reflexivity. 
+    + intros. rewrite (proj1 instantiate_hom). simpl. reflexivity.
+  - rewrite (fold_left_hom _
+            (fun (bod : Term) (ndx : nat) =>
+         instantiate (TFix (dcons n (strip t0) n0 (stripDs dts)) ndx) 0 bod)).
+    + rewrite dlength_hom. rewrite (proj1 instantiate_hom).
+      rewrite tcons_hom. reflexivity.
+    + intros. rewrite (proj1 instantiate_hom).
+      rewrite <- (dcons_hom _ L1.term.prop). simpl. reflexivity.
+Qed.
+
+Lemma whFixStep_hom:
+  forall dts m args,
+    optStrip (L1.term.whFixStep dts m args) =
+    whFixStep (stripDs dts) m (strips args).
+Proof.
+  intros dts m args.
+  unfold L1.term.whFixStep, whFixStep.
+  case_eq (L1.term.dnthBody m dts); intros.
+  - rewrite optStrip_hom. rewrite <- pre_whFixStep_hom.
+    rewrite <- dnthBody_hom. rewrite H. simpl. reflexivity.
+  - rewrite <- dnthBody_hom. rewrite H. reflexivity.
+Qed.
+
+
+(** The goal is to prove that if [wndEval.wndEval p t s] (unstripped),
+*** then [wndEval (stripEnv p) (strip t) (strip s)] (stripped).
+*** However the unstripped language has steps in type fields where the 
+*** stripped language can make no step.  Thus we need "reflexive closure",
+*** allowing null steps for the stripped language.
+**)
+Inductive wndEvalRC: environ -> Term -> Term -> Prop :=
+| wERCrfl: forall p t, wndEvalRC p t t
+| wERCstep: forall p t s, wndEval p t s -> wndEvalRC p t s.
+
+Inductive wndEvalsRC: environ -> Terms -> Terms -> Prop :=
+| wEsRCrfl: forall p ts, wndEvalsRC p ts ts
+| wEsRCstep: forall p ts ss, wndEvals p ts ss -> wndEvalsRC p ts ss.
+
+Inductive WcbvEvalRC: environ -> Term -> Term -> Prop :=
+| WcERCrfl: forall p t, WcbvEvalRC p t t
+| WcERCstep: forall p t s, WcbvEval p t s -> WcbvEvalRC p t s.
+
+Inductive WcbvEvalsRC: environ -> Terms -> Terms -> Prop :=
+| WcEsRCrfl: forall p ts, WcbvEvalsRC p ts ts
+| WcEsRCstep: forall p ts ss, WcbvEvals p ts ss -> WcbvEvalsRC p ts ss.
+
+Theorem L1wcbvEval_strip_L2WcbvEval:
+  forall p, L1.program.WFaEnv p ->
+    (forall t s, L1.wcbvEval.WcbvEval p t s -> L1.term.WFapp t ->
+          WcbvEval (stripEnv p) (strip t) (strip s)) /\
+    (forall ts ss, L1.wcbvEval.WcbvEvals p ts ss -> L1.term.WFapps ts ->
+          WcbvEvals (stripEnv p) (strips ts) (strips ss)).
+intros p hp.
+apply L1.wcbvEval.WcbvEvalEvals_ind; intros; try (solve [constructor]).
+- simpl. eapply wCast. inversion H0. intuition.
+- eapply wConst. 
+  + apply LookupDfn_hom. eassumption.
+  + apply H. assert (j:= L1.program.Lookup_pres_WFapp hp l). inversion_Clear j.
+    assumption.
+- rewrite TApp_hom. inversion H2. subst. eapply wAppLam.
+  + rewrite TLambda_hom in H. apply H. assumption.
+  + apply H0. assumption.
+  + rewrite whBetaStep_hom in H1. apply H1.
+    apply L1.term.whBetaStep_pres_WFapp; try assumption.
+    * assert (j:= proj1 (L1.wcbvEval.wcbvEval_pres_WFapp hp) _ _ w H7).
+      inversion j. assumption.
+    * apply (proj1 (L1.wcbvEval.wcbvEval_pres_WFapp hp) _ _ w0). assumption.
+- simpl. inversion H1. subst. eapply wLetIn.
+  + apply H. assumption.
+  + rewrite (proj1 instantiate_hom) in H0. apply H0.
+    apply L1.term.instantiate_pres_WFapp; try assumption.
+    * apply (proj1 (L1.wcbvEval.wcbvEval_pres_WFapp hp) _ _ w). assumption.
+- inversion_Clear H1.
+  assert (j:= proj1 (L1.wcbvEval.wcbvEval_pres_WFapp hp) _ _ w H6). 
+  inversion_Clear j.
+  rewrite TApp_hom. eapply wAppFix.
+  + rewrite TFix_hom in H. apply H. assumption.
+  + rewrite <- tcons_hom. rewrite <- whFixStep_hom. rewrite e. 
+    rewrite optStrip_hom. reflexivity.
+  + apply H0. refine (L1.term.whFixStep_pres_WFapp _ H2 _ e).
+    * constructor; assumption.
+- inversion_Clear H2. rewrite TApp_hom. rewrite TApp_hom. simpl. 
+  apply wAppCnstr; intuition.
+- inversion_Clear H2. rewrite TApp_hom. rewrite TApp_hom. simpl. 
+  apply wAppInd; intuition.
+- inversion_Clear H1. rewrite TCase_hom. eapply wCase0.
+  + simpl in H. apply H. assumption.
+  + rewrite <- tnil_hom. rewrite <- whCaseStep_hom. rewrite <- optStrip_hom.
+    apply f_equal. eassumption.
+  + apply H0. refine (L1.term.whCaseStep_pres_WFapp H7 _ _ e). constructor.
+- inversion_Clear H1. rewrite TCase_hom. simpl in H. eapply wCasen.
+  + apply H. assumption.
+  + rewrite <- tcons_hom. rewrite <- tskipn_hom. rewrite e. 
+    rewrite optStrips_hom. reflexivity.
+  + rewrite <- whCaseStep_hom. rewrite e0. rewrite optStrip_hom. reflexivity.
+  + apply H0. refine (L1.term.whCaseStep_pres_WFapp H7 _ _ e0). 
+    refine (L1.term.tskipn_pres_WFapp _ _ e).
+    assert (j: L1.term.WFapp (L1.term.TApp (L1.term.TConstruct i n) arg args)).
+    { refine (proj1 (L1.wcbvEval.wcbvEval_pres_WFapp hp) _ _ _ _).
+      apply mch. assumption. assumption. }
+    inversion_clear j.
+    constructor; assumption.
+- inversion_Clear H1. rewrite tcons_hom. rewrite tcons_hom.
+  constructor; intuition.
+Qed.
+
+Print Assumptions L1wcbvEval_strip_L2WcbvEval.
+
+Function unstrip (t:Term) : L1Term :=
+  match t with
+    | TRel n => L1.term.TRel n
+    | TSort s => L1.term.TSort s
+    | TCast t => L1.term.TCast (unstrip t) Cast L1.term.prop
+    | TProd nm bod => L1.term.TProd nm L1.term.prop (unstrip bod)
+    | TLambda nm bod => L1.term.TLambda nm L1.term.prop (unstrip bod)
+    | TLetIn nm dfn bod =>
+           L1.term.TLetIn nm (unstrip dfn) L1.term.prop (unstrip bod)
+    | TApp fn arg args =>
+           L1.term.TApp (unstrip fn) (unstrip arg) (unstrips args)
+    | TConst nm => L1.term.TConst nm
+    | TInd i => L1.term.TInd i
+    | TConstruct i m => L1.term.TConstruct i m
+    | TCase n mch brs =>
+           L1.term.TCase n L1.term.prop (unstrip mch) (unstrips brs)
+    | TFix ds n => L1.term.TFix (unstripDs ds) n
+  end
+with unstrips (ts:Terms) : L1Terms := 
+  match ts with
+    | tnil => L1.term.tnil
+    | tcons t ts => L1.term.tcons (unstrip t) (unstrips ts)
+  end
+with unstripDs (ts:Defs) : L1Defs := 
+  match ts with
+    | dnil => L1.term.dnil
+    | dcons nm t m ds =>
+           L1.term.dcons nm L1.term.prop (unstrip t) m (unstripDs ds)
+  end.
+
+Lemma strip_leftInv_unstrip:
+  (forall (t:Term), strip (unstrip t) = t) /\
+  (forall ts:Terms, strips (unstrips ts) = ts) /\
+  (forall ds:Defs, stripDs (unstripDs ds) = ds).
+Proof.
+  apply TrmTrmsDefs_ind; simpl; intros;
+  try reflexivity; try (rewrite H; reflexivity);
+  try (rewrite H; rewrite H0; reflexivity);
+  try (rewrite H; rewrite H0; rewrite H1; reflexivity).
+Qed.
+
+Definition optUnstrip (t:option Term) : option L1Term :=
+  match t with
+    | None => None
+    | Some t => Some (unstrip t)
+  end.
+Definition optUnstrips (ts:option Terms) : option L1Terms :=
+  match ts with
+    | None => None
+    | Some ts => Some (unstrips ts)
+  end.
+
+Lemma optUnstrip_unhom: forall y, optUnstrip (Some y) = Some (unstrip y).
+induction y; simpl; reflexivity.
+Qed.
+Lemma optUnstrips_unhom: forall y, optUnstrips (Some y) = Some (unstrips y).
+induction y; simpl; reflexivity.
+Qed.
+
+Function unstripCnstrs (cs:list Cnstr) : list L1.program.Cnstr :=
+  match cs with
+    | nil => nil
+    | cons (mkCnstr str arity) cs =>
+        cons (L1.program.mkCnstr str arity) (unstripCnstrs cs)
+  end.
+Function unstripItyPack (its:itypPack) : L1.program.itypPack :=
+  match its with
+    | nil => nil
+    | (mkItyp str itps) :: itpacks =>
+         (L1.program.mkItyp str (unstripCnstrs itps)) ::
+                           unstripItyPack itpacks
+  end.
+Function unstripEc (ec:envClass) : L1.program.envClass :=
+  match ec with
+    | ecTrm t => L1.program.ecTrm (unstrip t)
+    | ecTyp itp => L1.program.ecTyp (unstripItyPack itp)
+  end.
+Fixpoint unstripEnv (p:environ) : L1.program.environ :=
+  match p with
+    | nil => nil
+    | cons (nm, ec) q => cons (nm, (unstripEc ec)) (unstripEnv q)
+  end.
+
+
+Lemma Lam_strip_inv:
+  forall nm bod s, TLambda nm bod = strip s ->
+   exists sty sbod, 
+     (L1.term.TLambda nm sty sbod) = s /\ bod = strip sbod.
+Proof.
+  intros nm bod s; induction s; simpl; intros h; try discriminate.
+  - myInjection h. exists s1, s2. intuition. 
+Qed.
+
+Lemma L1WFapp_L2WFapp:
+  (forall t, L1.term.WFapp t -> WFapp (strip t)) /\
+  (forall ts, L1.term.WFapps ts -> WFapps (strips ts)) /\
+  (forall ds, L1.term.WFappDs ds -> WFappDs (stripDs ds)).
+Proof.
+  apply L1.term.WFappTrmsDefs_ind; simpl; constructor; auto.
+  - intros h. elim H. apply isApp_hom. assumption.
+Qed.
+
+
+Lemma L2WFapp_L1WFapp:
+  (forall t, WFapp t -> L1.term.WFapp (unstrip t)) /\
+  (forall ts, WFapps ts -> L1.term.WFapps (unstrips ts)) /\
+  (forall ds, WFappDs ds -> L1.term.WFappDs (unstripDs ds)).
+Proof.
+  apply WFappTrmsDefs_ind; simpl; intros; try (solve [constructor]);
+  try (solve [constructor; try assumption; constructor]).
+  - constructor; try assumption.
+    + intros h. elim H. destruct h as [x0 [x1 [x2 j]]].
+      assert (k:= f_equal strip j).
+      rewrite (proj1 (strip_leftInv_unstrip)) in k. rewrite k. simpl.
+      exists (strip x0), (strip x1), (strips x2). reflexivity.
+Qed.
+
+
+Lemma L1WFaEnv_L2WFaEnv:
+  forall p:L1.program.environ, L1.program.WFaEnv p -> WFaEnv (stripEnv p).
+Proof.
+  induction 1; simpl; constructor.
+  - inversion H; destruct ec; simpl; try discriminate.
+    + constructor. apply (proj1 (L1WFapp_L2WFapp)). assumption.
+    + constructor.
+  - assumption.
+Qed.
+
+Lemma Lookup_unhom:
+ forall nm p ec, 
+   Lookup nm p ec -> L1.program.Lookup nm (unstripEnv p) (unstripEc ec).
+Proof.
+  induction 1; destruct t; simpl.
+  - constructor.
+  - constructor.
+  - constructor; assumption.
+  - constructor; assumption.
+Qed.
+
+Lemma tappend_unhom:
+  forall ts us,
+    unstrips (tappend ts us) = L1.term.tappend (unstrips ts) (unstrips us).
+ Proof.
+   induction ts; intros us; simpl; try reflexivity.
+   - rewrite IHts. reflexivity.
+Qed.
+
+Lemma mkApp_unhom:
+  forall fn args,
+    unstrip (mkApp fn args) = L1.term.mkApp (unstrip fn) (unstrips args).
+Proof.
+  induction fn; induction args; simpl; try reflexivity.
+  - rewrite tappend_tnil. rewrite L1.term.tappend_tnil. reflexivity.
+  - rewrite tappend_unhom. simpl. reflexivity.
+Qed.
+
+Lemma dlength_unhom:
+  forall ds, dlength ds = L1.term.dlength (unstripDs ds).
+Proof.
+  induction ds; simpl.
+  - reflexivity.
+  - rewrite IHds. reflexivity.
+Qed.
+
+Lemma tcons_unhom:
+  forall t ts,
+    unstrips (tcons t ts) = L1.term.tcons (unstrip t) (unstrips ts).
+Proof.
+  reflexivity.
+Qed.
+
+Lemma dcons_unhom:
+  forall nm bod rarg ds,
+    unstripDs (dcons nm bod rarg ds) =
+    L1.term.dcons nm L1.term.prop (unstrip bod) rarg (unstripDs ds).
+reflexivity.
+Qed.
+
+
+Lemma instantiate_unhom: 
+  (forall bod tin ni,
+    unstrip (instantiate tin ni bod) =
+    L1.term.instantiate (unstrip tin) ni (unstrip bod)) /\
+  (forall bods tin ni,
+    unstrips (instantiates tin ni bods) =
+    L1.term.instantiates (unstrip tin) ni (unstrips bods)) /\
+  (forall ds tin ni,
+    unstripDs (instantiateDefs tin ni ds) =
+    L1.term.instantiateDefs (unstrip tin) ni (unstripDs ds)).
+Proof.
+  apply TrmTrmsDefs_ind; intros;
+  try (solve [unfold instantiate, L1.term.instantiate; simpl; reflexivity]).
+  - destruct (lt_eq_lt_dec n ni) as [[j1|j2]|j3];
+    unfold instantiate, L1.term.instantiate; simpl.
+    + rewrite (proj1 (nat_compare_gt _ _) j1). reflexivity.
+    + subst. rewrite (proj2 (nat_compare_eq_iff ni ni)); try reflexivity.
+      rewrite mkApp_unhom. simpl. reflexivity.
+    + rewrite (proj1 (nat_compare_lt _ _) j3). reflexivity.
+  - change (unstrip (TCast (instantiate tin ni t)) =
+            L1.term.TCast
+              (L1.term.instantiate (unstrip tin) ni (unstrip t))
+              Cast L1.term.prop).
+    rewrite <- H. simpl. reflexivity.
+  - change (unstrip (TProd n (instantiate tin (S ni) t)) =
+            L1.term.TProd n L1.term.prop
+                          (L1.term.instantiate (unstrip tin) (S ni)
+                                               (unstrip t))).
+    rewrite <- H. simpl. reflexivity.
+  - change (unstrip (TLambda n (instantiate tin (S ni) t)) =
+            L1.term.TLambda n L1.term.prop
+                            (L1.term.instantiate (unstrip tin) (S ni)
+                                                 (unstrip t))).
+    rewrite <- H. simpl. reflexivity.
+  - change (unstrip (TLetIn n (instantiate tin ni t)
+                            (instantiate tin (S ni) t0)) =
+            L1.term.TLetIn n (L1.term.instantiate
+                                (unstrip tin) ni (unstrip t))
+                           L1.term.prop
+                           (L1.term.instantiate
+                              (unstrip tin) (S ni) (unstrip t0))).
+    rewrite <- H. rewrite <- H0. simpl. reflexivity.
+  - change (unstrip (mkApp (instantiate tin ni t)
+                           (tcons (instantiate tin ni t0)
+                                  (instantiates tin ni t1))) =
+            L1.term.mkApp (L1.term.instantiate (unstrip tin) ni (unstrip t))
+                          (L1.term.tcons 
+                             (L1.term.instantiate 
+                                (unstrip tin) ni (unstrip t0))
+                             (L1.term.instantiates
+                                (unstrip tin) ni (unstrips t1)))).
+    rewrite <- H. rewrite <- H0. rewrite <- H1. simpl.
+    rewrite mkApp_unhom. reflexivity.
+  - change (unstrip (TCase n (instantiate tin ni t)
+                           (instantiates tin ni t0)) =
+            L1.term.TCase n L1.term.prop
+                          (L1.term.instantiate (unstrip tin) ni (unstrip t))
+                          (L1.term.instantiates (unstrip tin) ni
+                                                (unstrips t0))).
+    rewrite <- H. rewrite <- H0. simpl. reflexivity.
+  - change (unstrip (TFix (instantiateDefs tin (ni + dlength d) d) n) =
+            L1.term.TFix
+              (L1.term.instantiateDefs (unstrip tin)
+                                       (ni + L1.term.dlength (unstripDs d))
+                                       (unstripDs d)) n).
+    rewrite <- H. rewrite dlength_unhom. simpl. reflexivity.
+  - change (unstrips (tcons (instantiate tin ni t)
+                            (instantiates tin ni t0)) =
+            L1.term.tcons (L1.term.instantiate (unstrip tin) ni (unstrip t))
+                          (L1.term.instantiates (unstrip tin) ni
+                                                (unstrips t0))).
+    rewrite <- H. rewrite <- H0. simpl. reflexivity.
+  - change (unstripDs (dcons n (instantiate tin ni t) n0
+                            (instantiateDefs tin ni d)) =
+            L1.term.dcons n L1.term.prop
+                          (L1.term.instantiate (unstrip tin) ni (unstrip t))
+                          n0
+                          (L1.term.instantiateDefs (unstrip tin) ni
+                                                   (unstripDs d))).
+    rewrite <- H. rewrite <- H0. simpl. reflexivity.
+Qed.
+
+Lemma whBetaStep_unhom:
+  forall bod a1 args,
+    unstrip (whBetaStep bod a1 args) =
+    L1.term.whBetaStep (unstrip bod) (unstrip a1) (unstrips args).
+Proof.
+  intros bod a1 args. unfold whBetaStep, L1.term.whBetaStep.
+  rewrite <- (proj1 instantiate_unhom). rewrite <- mkApp_unhom. reflexivity.
+Qed.
+
+Lemma dnthBody_unhom:
+  forall m ds,
+    optUnstrip (dnthBody m ds) = L1.term.dnthBody m (unstripDs ds).
+Proof.
+  induction m; induction ds; try intuition.
+  - simpl. intuition.
+Qed.
+
+Lemma fold_left_unhom:
+forall (F:Term -> nat -> Term) 
+       (unstripF:L1Term -> nat -> L1Term) (ns:list nat) (t:Term),
+  (forall (s:Term) (n:nat), unstrip (F s n) = unstripF (unstrip s) n) ->
+  unstrip (fold_left F ns t) = fold_left unstripF ns (unstrip t).
+induction ns; intros t h.
+- intuition.
+- simpl. rewrite IHns.
+  + rewrite h. reflexivity.
+  + assumption.
+Qed.
+
+Lemma pre_whFixStep_unhom:
+  forall body dts args,
+    unstrip (pre_whFixStep body dts args) = 
+    L1.term.pre_whFixStep (unstrip body) (unstripDs dts) (unstrips args).
+Proof. 
+  intros body dts args.
+  destruct dts, args; unfold pre_whFixStep, L1.term.pre_whFixStep;
+  simpl; rewrite mkApp_unhom; try reflexivity.
+  - rewrite (fold_left_unhom _ 
+         (fun (bod : L1.term.Term) (ndx : nat) =>
+            L1.term.instantiate
+              (L1.term.TFix (unstripDs (dcons n t n0 dts)) ndx) 0 bod)).
+    + rewrite <- dcons_unhom. rewrite (proj1 instantiate_unhom). simpl.
+      rewrite dlength_unhom. reflexivity.
+    + intros. simpl. rewrite (proj1 instantiate_unhom). simpl.
+      reflexivity.
+  - rewrite (fold_left_unhom _ 
+         (fun (bod : L1.term.Term) (ndx : nat) =>
+            L1.term.instantiate
+              (L1.term.TFix (unstripDs (dcons n t n0 dts)) ndx) 0 bod)).
+    + rewrite dlength_unhom. rewrite (proj1 instantiate_unhom).
+      rewrite dcons_unhom. rewrite tcons_unhom. reflexivity.
+    + intros. rewrite (proj1 instantiate_unhom).
+      rewrite dcons_unhom. reflexivity.
+Qed.
+
+Lemma whFixStep_unhom:
+  forall dts m args,
+    optUnstrip (whFixStep dts m args) =
+    L1.term.whFixStep (unstripDs dts) m (unstrips args).
+Proof.
+  intros dts m args.
+  unfold L1.term.whFixStep, whFixStep. case_eq (dnthBody m dts); intros.
+  - rewrite optUnstrip_unhom. rewrite pre_whFixStep_unhom.
+    rewrite <- dnthBody_unhom. rewrite H. simpl. reflexivity.
+  - rewrite <- dnthBody_unhom. rewrite H. reflexivity.
+Qed.
+
+Lemma tnth_unhom:
+ forall ts n, optUnstrip (tnth n ts) = L1.term.tnth n (unstrips ts).
+Proof.
+  induction ts; simpl; intros n; case n; try reflexivity; trivial.
+Qed. 
+
+Lemma whCaseStep_unhom:
+forall n ts brs,
+  optUnstrip (whCaseStep n ts brs) = 
+  L1.term.whCaseStep n (unstrips ts) (unstrips brs).
+Proof.
+  destruct n, brs; intros; simpl; try reflexivity.
+  - unfold whCaseStep. simpl. rewrite mkApp_unhom. reflexivity.
+  - unfold whCaseStep. unfold L1.term.whCaseStep. simpl.
+    rewrite <- tnth_unhom. destruct (tnth n brs); simpl.
+    + rewrite mkApp_unhom. reflexivity.
+    + reflexivity. 
+Qed.
+
+Lemma tskipn_unhom:
+  forall ts n, optUnstrips (tskipn n ts) = L1.term.tskipn n (unstrips ts).
+induction ts; simpl; intros n; case n; try reflexivity; trivial.
+Qed.
+
+
+(** L2 WcbvEval is sound for L1 WcbvEval **)
+Theorem L2WcbvEval_L1WcbvEval:
+  forall p,
+    (forall t s, WcbvEval p t s ->
+     L1.wcbvEval.WcbvEval (unstripEnv p) (unstrip t) (unstrip s)) /\
+    (forall ts ss, WcbvEvals p ts ss ->
+     L1.wcbvEval.WcbvEvals (unstripEnv p) (unstrips ts) (unstrips ss)).
+Proof.
+  intros p.
+  apply WcbvEvalEvals_ind; simpl; intros; try (solve [constructor]);
+  try (solve [constructor; constructor]);
+  try (solve [constructor; assumption]).
+  - eapply L1.wcbvEval.wConst; try eassumption. apply (Lookup_unhom l).
+  - eapply L1.wcbvEval.wAppLam; try eassumption.
+    + rewrite <- whBetaStep_unhom. assumption.
+  - eapply L1.wcbvEval.wLetIn; try eassumption.
+    + rewrite <- (proj1 instantiate_unhom). assumption.
+  - eapply L1.wcbvEval.wAppFix; try eassumption.
+    + rewrite <- tcons_unhom. rewrite <- whFixStep_unhom.
+      rewrite <- optUnstrip_unhom. apply f_equal. assumption.
+  - eapply L1.wcbvEval.wCase0; try eassumption.
+    + change (L1.term.whCaseStep n (unstrips tnil) (unstrips brs) =
+              Some (unstrip cs)).
+      rewrite <- whCaseStep_unhom. rewrite <- optUnstrip_unhom.
+      apply f_equal. assumption.
+  - eapply L1.wcbvEval.wCasen; try eassumption. 
+    + rewrite <- tcons_unhom. rewrite <- tskipn_unhom.
+      rewrite <- optUnstrips_unhom. apply f_equal. eassumption.
+    + rewrite <- whCaseStep_unhom. rewrite <- optUnstrip_unhom.
+      apply f_equal. assumption.
+Qed.
+
+
+(** NO?? strip throws away info **
+Goal
+  forall L2p p, L2p = stripEnv p ->
+    (forall L2t L2s, WcbvEval L2p L2t L2s ->
+     forall t, L2t = strip t -> forall s, L2s = strip s ->
+                                          L1.wcbvEval.WcbvEval p t s) /\
+    (forall L2ts L2ss, WcbvEvals L2p L2ts L2ss ->
+     forall ts, L2ts = strips ts -> forall ss, L2ss = strips ss ->
+                                          L1.wcbvEval.WcbvEvals p ts ss).
+Proof.
+  intros L2p p hp.
+  apply WcbvEvalEvals_ind; simpl; intros.
+  - destruct (Lam_strip_inv _ H) as [t0 [t1 [jtl jtr]]].
+    destruct (Lam_strip_inv _ H0) as [s0 [s1 [jsl jsr]]].
+    subst.
+
+
+WcbvEval (stripEnv p) (strip t) (strip s) -> 
+     L1.wcbvEval.WcbvEval p t s) /\
+    (forall ts ss, WcbvEvals (stripEnv p) (strips ts) (strips ss) ->
+     L1.wcbvEval.WcbvEvals p ts ss).
+Proof.
+
+Theorem L2WcbvEval_L1wndEval:
+  forall (p:L1.program.environ), L1.program.WFaEnv p ->
+    (forall t s, WcbvEval (stripEnv p) (strip t) (strip s) -> 
+                 L1.term.WFapp t -> L1.wndEval.wndEvalRTC p t s) /\
+    (forall ts ss, WcbvEvals (stripEnv p) (strips ts) (strips ss) ->
+                   L1.term.WFapps ts -> L1.wndEval.wndEvalsRTC p ts ss).
+**)
+
+
+
+
+(**** below here scratch ****
+Goal
+  forall (q:environ), WFaEnv q ->
+     forall p1, q = stripEnv p1 -> forall p2, q = stripEnv p2 ->
+  (forall (t x:Term), WcbvEval q t x -> 
+      forall t1, t = strip t1 -> forall t2, t = strip t2 -> 
+     forall s1 s2, L1.wcbvEval.WcbvEval p1 t1 s1 ->
+            L1.wcbvEval.WcbvEval p2 t2 s2 -> strip s1 = strip s2) /\
+  (forall (ts xs:Terms), WcbvEvals q ts xs -> 
+     forall t1s, ts = strips t1s -> forall t2s, ts = strips t2s -> 
+     forall s1s s2s, L1.wcbvEval.WcbvEvals p1 t1s s1s ->
+            L1.wcbvEval.WcbvEvals p2 t2s s2s -> strips s1s = strips s2s).
+Proof.
+Admitted.
+(***********
+  intros q hq p1 hp1 p2 hp2.
+  apply WcbvEvalEvals_ind; intros.
+  - destruct (Lam_strip_inv _ H) as [x1 [y1 [j1 k1]]]. clear H.
+    destruct (Lam_strip_inv _ H0) as [x2 [y2 [j2 k2]]]. clear H0.
+    subst.
+    refine (WcbvEval_single_valued _ _).
+    inversion H1. subst.
+    refine (proj1 (L1wcbvEval_strip_L2WcbvEval _) _ _ _ _).
+
+
+     (proj1 (L1wcbvEval_strip_L2WcbvEval _)).
+
+
+    refine (proj1 (L1wcbvEval_strip_L2WcbvEval _) _ _ _ _).
+
+
+
+Qed.
+
+***********)
+
+
+
+Theorem L2wcbvEval_strip_L1WcbvEval:
+  forall pp, WFaEnv pp -> forall p, pp = stripEnv p ->
+    (forall (tt ss:Term), WcbvEval pp tt ss -> WFapp tt ->
+     forall (t:L1Term), tt = strip t -> 
+       exists s:L1Term, ss = strip s /\ L1.wcbvEval.WcbvEval p t s)  /\
+    (forall tts sss, WcbvEvals pp tts sss -> WFapps tts ->
+     forall ts, tts = strips ts ->
+       exists ss:L1Terms, sss = strips ss /\ L1.wcbvEval.WcbvEvals p ts ss).
+Proof.
+
+
+Theorem L2wcbvEval_strip_L1WcbvEval:
+  forall pp, WFaEnv pp -> forall p, pp = stripEnv p ->
+    (forall (tt ss:Term), WcbvEval pp tt ss -> WFapp tt ->
+     forall (t:L1Term), tt = strip t -> 
+       exists s:L1Term, ss = strip s /\ L1.wcbvEval.WcbvEval p t s)  /\
+    (forall tts sss, WcbvEvals pp tts sss -> WFapps tts ->
+     forall ts, tts = strips ts ->
+       exists ss:L1Terms, sss = strips ss /\ L1.wcbvEval.WcbvEvals p ts ss).
+Proof.
+  intros pp hpp p hp. apply WcbvEvalEvals_ind; intros.
+  - destruct (Lam_strip_inv H0 _) as [x0 [x1 [j0 j1]]]. subst.
+    exists (L1.term.TLambda nm L1.term.prop x1). intuition.
+    apply L1.wcbvEval.wLam.
+
+
+    destruct (Lam_strip_inv _ H1) as [y0 [y1 [k0 k1]]].
+    subst. simpl in *. apply L1.wcbvEval.wLam.
+
+rewrite H1 in H0.
+
+
+(*************
+Lemma wndEval_types_irrelevant:
+  forall p,
+    (forall t s, L1.wndEval.wndEval p t s ->
+          wndEvalRC (stripEnv p) (strip t) (strip s)) /\
+    (forall ts ss, L1.wndEval.wndEvals p ts ss ->
+          wndEvalsRC (stripEnv p) (strips ts) (strips ss)).
+intros p. apply L1.wndEval.wndEvalEvals_ind; intros.
+- apply wERCstep. constructor. apply LookupDfn_hom. assumption.
+- apply wERCstep. simpl. rewrite whBetaStep_hom. apply sBeta.
+- apply wERCstep. simpl. rewrite (proj1 (instantiate_hom )).
+  apply sLetIn.
+- apply wERCstep. rewrite TCase_hom. apply sCase0.
+  assert (j: optStrip (L1.term.whCaseStep n L1.term.tnil brs) =
+             optStrip (Some s)).
+  apply f_equal. assumption.
+  simpl in j. rewrite <- j. rewrite whCaseStep_hom. reflexivity.
+- apply wERCstep. simpl. eapply sCasen.
+  rewrite <- tcons_hom. rewrite <- tskipn_hom. rewrite e. reflexivity.
+  rewrite <- whCaseStep_hom. rewrite e0. reflexivity.
+- apply wERCstep. rewrite TApp_hom. rewrite TFix_hom. apply sFix.
+  assert (j: optStrip (L1.term.whFixStep dts m (L1.term.tcons arg args)) = 
+             optStrip (Some s)).
+  apply f_equal. assumption.
+  simpl in j. rewrite <- j. rewrite whFixStep_hom. reflexivity.
+  intros h. simpl in h. destruct h as [x0 [x1 [x2 j]]]. discriminate.
+- simpl. apply wERCrfl.
+- rewrite mkApp_hom. rewrite tcons_hom. rewrite TApp_hom.
+
+- assert (j:= L1.term.mkApp_isApp r arg args).
+  destruct j as [x0 [x1 [x2 k]]]. rewrite k.
+  simpl.
+  inversion H. 
+  + rewrite mkApp_goodFn. HERE
+
+- rewrite mkApp_hom. rewrite tcons_hom. (* rewrite TApp_hom. *)
+  inversion H.
+  + rewrite mkApp_goodFn. simpl.
+    * constructor. rewrite TApp_hom. constructor.
+    * intros h. elim n. apply (proj1 (isApp_hom _)). assumption.
+  + apply wERCstep. apply sAppFn; assumption. 
+- rewrite TApp_hom. rewrite TApp_hom.
+  inversion_clear H. constructor.
+  + apply wERCstep; apply sAppArg; assumption. 
+- rewrite TApp_hom. rewrite TApp_hom. inversion_clear H. constructor.
+  + apply wERCstep. apply sAppArgs. assumption. 
+    (* no step for TProd or TLambda in stripped language *)
+- rewrite TProd_hom. rewrite TProd_hom. apply wERCrfl.
+- rewrite TLambda_hom. rewrite TLambda_hom. apply wERCrfl.
+- rewrite TLetIn_hom. rewrite TLetIn_hom. apply wERCrfl.
+- rewrite TLetIn_hom. rewrite TLetIn_hom. inversion_clear H. constructor.
+  + apply wERCstep. apply sLetInDef. assumption.
+- rewrite TCase_hom. rewrite TCase_hom. inversion_clear H. constructor.
+  + apply wERCrfl.
+- rewrite TCase_hom. rewrite TCase_hom. inversion_clear H. constructor.
+  + apply wERCstep. apply sCaseArg. assumption.
+- rewrite TCase_hom. rewrite TCase_hom. inversion_clear H. constructor.
+  + apply wERCstep. apply sCaseBrs. assumption.
+- rewrite tcons_hom. rewrite tcons_hom. inversion_clear H. constructor.
+  + apply wEsRCstep. apply saHd. assumption.
+- rewrite tcons_hom. rewrite tcons_hom. inversion_clear H. constructor.
+  + apply wEsRCstep. apply saTl. assumption.
+Qed.
+***********************)
+
+***)
