reify/template-coq-univ-is-type/test-suite/reflect.v
@@ -1,0 +1,8 @@
+Require Import Template.Template.
+Require Import String.
+
+Definition foo := 1 + 1.
+
+Quote Definition foo_syn := Eval cbv delta [ foo ] in foo.
+
+Make Definition foo_sem := Eval compute in foo_syn.
